Refactor conservation laws to make proof more maliable and managable.

hpaxos_liveness.thy
@@ -39,92 +39,8 @@ induction that the only way for this to happen is a proccess1a step.
 With appropriate assumptions, all proerties should continue to hold
 as well.
 *)
-lemma step_1a_only:
-  assumes "Spec f"
-      and "M1a b \<in> set (msgs (f i))"
-      and "is_safe a"
-      and "M1a b \<notin> set (known_msgs_acc (f i) a)"
-    shows "i < j \<and> M1a b \<in> set (known_msgs_acc (f j) a) \<longrightarrow>
-           (\<exists>k. i \<le> k \<and> k < j \<and> Process1a a (M1a b) (f k) (f (1 + k)))"
-proof (induction j)
-  case 0
-  then show ?case 
-    by fastforce
-next
-  case (Suc j)
-  show "i < Suc j \<and> M1a b \<in> set (known_msgs_acc (f (Suc j)) a) \<longrightarrow>
-                 (\<exists>k\<ge>i. k < Suc j \<and> Process1a a (M1a b) (f k) (f (1 + k)))"
-  proof (cases "M1a b \<in> set (known_msgs_acc (f j) a)")
-    case True
-    then show ?thesis
-      using Suc assms(4) less_Suc_eq by blast
-  next
-    case False
-    then show ?thesis
-    proof (clarify)
-      assume "i < Suc j"
-         and "M1a b \<in> set (known_msgs_acc (f (Suc j)) a)"
-      have "Next (f j) (f (Suc j))"
-        by (metis False Spec.elims(2) \<open>M1a b \<in> set (known_msgs_acc (f (Suc j)) a)\<close> assms(1))
-      then have "\<not> (ProposerSendAction (f j) (f (Suc j)))"
-        by (metis False ProposerSendAction.elims(2) Send1a.elims(2) \<open>M1a b \<in> set (known_msgs_acc (f (Suc j)) a)\<close> ext_inject surjective update_convs(1))
-      have "\<forall> ln m. \<not> (LearnerRecv ln m (f j) (f (Suc j)))"
-        by (smt (verit, ccfv_SIG) False LearnerRecv.simps \<open>M1a b \<in> set (known_msgs_acc (f (Suc j)) a)\<close> ext_inject surjective update_convs(3))
-      have "\<forall> ln blt val. \<not> (LearnerDecide ln blt val (f j) (f (Suc j)))"
-        using False \<open>M1a b \<in> set (known_msgs_acc (f (Suc j)) a)\<close> by force
-      then have "\<forall>a. \<not> (LearnerProcessAction (f j) (f (Suc j)))"
-        by (meson LearnerAction.elims(2) LearnerProcessAction.elims(1) \<open>\<forall>ln m. \<not> LearnerRecv ln m (f j) (f (Suc j))\<close>)
-      have "\<forall>a. \<not> (FakeSend1b a (f j) (f (Suc j)))"
-        by (metis FakeSend1b.elims(1) False \<open>M1a b \<in> set (known_msgs_acc (f (Suc j)) a)\<close> ext_inject surjective update_convs(1))
-      have "\<forall>a. \<not> (FakeSend2a a (f j) (f (Suc j)))"
-        by (metis FakeSend2a.simps False \<open>M1a b \<in> set (known_msgs_acc (f (Suc j)) a)\<close> ext_inject surjective update_convs(1))
-      then have "\<not> (FakeAcceptorAction (f j) (f (Suc j)))"
-        using FakeAcceptorAction.simps \<open>\<forall>a. \<not> FakeSend1b a (f j) (f (Suc j))\<close> by presburger
-      then have "AcceptorProcessAction (f j) (f (Suc j))"
-        by (meson LearnerAction.elims(2) LearnerProcessAction.elims(2) Next.simps \<open>Next (f j) (f (Suc j))\<close> \<open>\<forall>ln blt val. \<not> LearnerDecide ln blt val (f j) (f (Suc j))\<close> \<open>\<forall>ln m. \<not> LearnerRecv ln m (f j) (f (Suc j))\<close> \<open>\<not> ProposerSendAction (f j) (f (Suc j))\<close>)
-      have "\<forall> A m. a \<noteq> A \<longrightarrow> \<not> (Process1a A m (f j) (f (Suc j)))"
-        by (metis False Process1a.elims(2) Store_acc.elims(2) \<open>M1a b \<in> set (known_msgs_acc (f (Suc j)) a)\<close>)
-      have "\<forall> A m. a \<noteq> A \<longrightarrow> \<not> (Process1b A m (f j) (f (Suc j)))"
-        by (metis False Process1b.elims(2) Store_acc.elims(2) \<open>M1a b \<in> set (known_msgs_acc (f (Suc j)) a)\<close>)
-      have "\<forall> a. \<not> (Process1bLearnerLoopDone a (f j) (f (Suc j)))"
-        using False \<open>M1a b \<in> set (known_msgs_acc (f (Suc j)) a)\<close> by force
-      have "\<forall> ln. \<not> (Process1bLearnerLoopStep a ln (f j) (f (Suc j)))"
-        unfolding Process1bLearnerLoopStep.simps
-        by (smt (verit, ccfv_SIG) False PreMessage.distinct(3) Store_acc.elims(2) \<open>M1a b \<in> set (known_msgs_acc (f (Suc j)) a)\<close> set_ConsD)  
-      then have "\<forall> A. a \<noteq> A \<longrightarrow> \<not> AcceptorAction A (f j) (f (Suc j))"
-      proof -
-        { fix aa :: Acceptor
-          have "known_msgs_acc (f (Suc j)) \<noteq> known_msgs_acc (f j) \<and> known_msgs_acc (f (Suc j)) a \<noteq> known_msgs_acc (f j) a"
-            using False \<open>M1a b \<in> set (known_msgs_acc (f (Suc j)) a)\<close> by fastforce
-          then have "aa = a \<or> \<not> AcceptorAction aa (f j) (f (Suc j))"
-            by (metis (full_types) AcceptorAction.elims(2) Process1bLearnerLoop.elims(2) Process1bLearnerLoopStep.elims(2) Store_acc.elims(2) \<open>\<forall>A m. a \<noteq> A \<longrightarrow> \<not> Process1a A m (f j) (f (Suc j))\<close> \<open>\<forall>A m. a \<noteq> A \<longrightarrow> \<not> Process1b A m (f j) (f (Suc j))\<close> \<open>\<forall>a. \<not> Process1bLearnerLoopDone a (f j) (f (Suc j))\<close>) }
-        then show ?thesis
-          by (metis (no_types))
-      qed
-      then have "AcceptorAction a (f j) (f (Suc j))"
-        by (metis AcceptorProcessAction.simps \<open>AcceptorProcessAction (f j) (f (Suc j))\<close>)
-      have "\<forall> m. (M1a b) \<noteq> m \<longrightarrow> \<not> (Process1a a m (f j) (f (Suc j)))"
-        unfolding Process1a.simps
-        by (metis False Store_acc.elims(2) \<open>M1a b \<in> set (known_msgs_acc (f (Suc j)) a)\<close> set_ConsD)
-      have "\<not> (Process1b a (M1a b) (f j) (f (Suc j)))"
-        by simp
-      have "\<forall> m. (M1a b) \<noteq> m \<longrightarrow> \<not> (Process1b a m (f j) (f (Suc j)))"
-        unfolding Process1b.simps
-        by (metis (no_types, lifting) False Store_acc.elims(2) \<open>M1a b \<in> set (known_msgs_acc (f (Suc j)) a)\<close> set_ConsD)
-      then have "\<forall> m. \<not> (Process1b a m (f j) (f (Suc j)))"
-        by (metis \<open>\<not> Process1b a (M1a b) (f j) (f (Suc j))\<close>)
-      then have "Process1a a (M1a b) (f j) (f (Suc j))"
-        by (metis AcceptorAction.elims(2) Process1bLearnerLoop.elims(2) \<open>AcceptorAction a (f j) (f (Suc j))\<close> \<open>\<forall>a. \<not> Process1bLearnerLoopDone a (f j) (f (Suc j))\<close> \<open>\<forall>ln. \<not> Process1bLearnerLoopStep a ln (f j) (f (Suc j))\<close> \<open>\<forall>m. M1a b \<noteq> m \<longrightarrow> \<not> Process1a a m (f j) (f (Suc j))\<close>)
-      then show "\<exists>k\<ge>i. k < Suc j \<and> Process1a a (M1a b) (f k) (f (1 + k))"
-        by (metis \<open>i < Suc j\<close> lessI less_Suc_eq_le plus_1_eq_Suc)
-    qed
-  qed
-qed
-
 lemma step_1a_side:
   assumes "Spec f"
-      and "M1a b \<in> set (msgs (f i))"
-      and "is_safe a"
       and "M1a b \<notin> set (known_msgs_acc (f i) a)"
     shows "i < j \<and> M1a b \<in> set (known_msgs_acc (f j) a) \<longrightarrow>
            (\<exists>k. i \<le> k \<and> k < j \<and> 
@@ -141,7 +57,7 @@ next
   proof (cases "M1a b \<in> set (known_msgs_acc (f j) a)")
     case True
     then show ?thesis
-      using Suc assms(4) less_Suc_eq by blast
+      using Suc assms(2) less_Suc_eq by blast
   next
     case False
     then show ?thesis
@@ -207,108 +123,238 @@ next
   qed
 qed
 
+lemma step_1b_side:
+  assumes "Spec f"
+      and "m \<notin> set (known_msgs_acc (f i) a)"
+      and "type m = T1b"
+    shows "i < j \<and> m \<in> set (known_msgs_acc (f j) a) \<longrightarrow>
+           (\<exists>k. i \<le> k \<and> k < j \<and> 
+              m \<notin> set (known_msgs_acc (f k) a)
+            \<and> Process1b a m (f k) (f (1 + k)))"
+proof (induction j)
+  case 0
+  then show ?case 
+    by fastforce
+next
+  case (Suc j)
+  show "i < Suc j \<and> m \<in> set (known_msgs_acc (f (Suc j)) a) \<longrightarrow>
+                 (\<exists>k\<ge>i. k < Suc j \<and> m \<notin> set (known_msgs_acc (f k) a) \<and> Process1b a m (f k) (f (1 + k)))"
+  proof (cases "m \<in> set (known_msgs_acc (f j) a)")
+    case True
+    then show ?thesis
+      using Suc assms(2) assms(3) less_Suc_eq by blast
+  next
+    case False
+    have "(\<forall>m \<in> set (known_msgs_acc (f (Suc j)) a). type m = T1b \<longrightarrow> m \<in> set (known_msgs_acc (f j) a)) \<longrightarrow> ?thesis"
+      using False assms(3) by blast
+    show ?thesis
+    proof (clarify)
+      assume "i < Suc j"
+         and "m \<in> set (known_msgs_acc (f (Suc j)) a)"
+      then have kne: "known_msgs_acc (f j) a \<noteq> known_msgs_acc (f (Suc j)) a"
+        using False by force
+      have "Next (f j) (f (Suc j))"
+        by (metis False Spec.elims(2) \<open>m \<in> set (known_msgs_acc (f (Suc j)) a)\<close> assms(1))
+      then have "\<not> (ProposerSendAction (f j) (f (Suc j)))"
+        by (metis False ProposerSendAction.elims(2) Send1a.elims(2) \<open>m \<in> set (known_msgs_acc (f (Suc j)) a)\<close> ext_inject surjective update_convs(1))
+      have "\<forall> ln m. \<not> (LearnerRecv ln m (f j) (f (Suc j)))"
+        by (smt (verit, ccfv_SIG) False LearnerRecv.simps \<open>m \<in> set (known_msgs_acc (f (Suc j)) a)\<close> ext_inject surjective update_convs(3))
+      have "\<forall> ln blt val. \<not> (LearnerDecide ln blt val (f j) (f (Suc j)))"
+        using False \<open>m \<in> set (known_msgs_acc (f (Suc j)) a)\<close> by force
+      then have "\<forall>a. \<not> (LearnerProcessAction (f j) (f (Suc j)))"
+        by (meson LearnerAction.elims(2) LearnerProcessAction.elims(1) \<open>\<forall>ln m. \<not> LearnerRecv ln m (f j) (f (Suc j))\<close>)
+      have "\<forall>a. \<not> (FakeSend1b a (f j) (f (Suc j)))"
+        by (metis FakeSend1b.elims(1) False \<open>m \<in> set (known_msgs_acc (f (Suc j)) a)\<close> ext_inject surjective update_convs(1))
+      have "\<forall>a. \<not> (FakeSend2a a (f j) (f (Suc j)))"
+        by (metis FakeSend2a.simps False \<open>m \<in> set (known_msgs_acc (f (Suc j)) a)\<close> ext_inject surjective update_convs(1))
+      then have "\<not> (FakeAcceptorAction (f j) (f (Suc j)))"
+        using FakeAcceptorAction.simps \<open>\<forall>a. \<not> FakeSend1b a (f j) (f (Suc j))\<close> by presburger
+      then have "AcceptorProcessAction (f j) (f (Suc j))"
+        by (meson LearnerAction.elims(2) LearnerProcessAction.elims(2) Next.simps \<open>Next (f j) (f (Suc j))\<close> \<open>\<forall>ln blt val. \<not> LearnerDecide ln blt val (f j) (f (Suc j))\<close> \<open>\<forall>ln m. \<not> LearnerRecv ln m (f j) (f (Suc j))\<close> \<open>\<not> ProposerSendAction (f j) (f (Suc j))\<close>)
+      have "\<forall> A m. a \<noteq> A \<longrightarrow> \<not> (Process1a A m (f j) (f (Suc j)))"
+        by (metis False Process1a.elims(2) Store_acc.elims(2) \<open>m \<in> set (known_msgs_acc (f (Suc j)) a)\<close>)
+      have "\<forall> A m. a \<noteq> A \<longrightarrow> \<not> (Process1b A m (f j) (f (Suc j)))"
+        by (metis False Process1b.elims(2) Store_acc.elims(2) \<open>m \<in> set (known_msgs_acc (f (Suc j)) a)\<close>)
+      have "\<forall> a. \<not> (Process1bLearnerLoopDone a (f j) (f (Suc j)))"
+        using False \<open>m \<in> set (known_msgs_acc (f (Suc j)) a)\<close> by force
+      have "\<forall> ln. \<not> (Process1bLearnerLoopStep a ln (f j) (f (Suc j)))"
+        by (smt (verit) False MessageType.distinct(5) Process1bLearnerLoopStep.elims(2) Store_acc.elims(2) \<open>m \<in> set (known_msgs_acc (f (Suc j)) a)\<close> assms(3) set_ConsD type.simps(3))
+      then have "\<forall> A. a \<noteq> A \<longrightarrow> \<not> AcceptorAction A (f j) (f (Suc j))"
+      proof -
+        { fix aa :: Acceptor
+          have "known_msgs_acc (f (Suc j)) \<noteq> known_msgs_acc (f j) \<and> known_msgs_acc (f (Suc j)) a \<noteq> known_msgs_acc (f j) a"
+            using False \<open>m \<in> set (known_msgs_acc (f (Suc j)) a)\<close> by fastforce
+          then have "aa = a \<or> \<not> AcceptorAction aa (f j) (f (Suc j))"
+            by (metis (full_types) AcceptorAction.elims(2) Process1bLearnerLoop.elims(2) Process1bLearnerLoopStep.elims(2) Store_acc.elims(2) \<open>\<forall>A m. a \<noteq> A \<longrightarrow> \<not> Process1a A m (f j) (f (Suc j))\<close> \<open>\<forall>A m. a \<noteq> A \<longrightarrow> \<not> Process1b A m (f j) (f (Suc j))\<close> \<open>\<forall>a. \<not> Process1bLearnerLoopDone a (f j) (f (Suc j))\<close>) }
+        then show ?thesis
+          by (metis (no_types))
+      qed
+      then have "AcceptorAction a (f j) (f (Suc j))"
+        by (metis AcceptorProcessAction.simps \<open>AcceptorProcessAction (f j) (f (Suc j))\<close>)
+      have "\<forall>m. \<not> (Process1a a m (f j) (f (Suc j)))"
+        by (metis False MessageType.distinct(1) Process1a.elims(2) Store_acc.elims(2) \<open>m \<in> set (known_msgs_acc (f (Suc j)) a)\<close> assms(3) set_ConsD)
+      have "\<forall> M. m \<noteq> M \<longrightarrow> \<not> (Process1b a M (f j) (f (Suc j)))"
+        unfolding Process1b.simps
+        by (metis False Store_acc.elims(2) \<open>m \<in> set (known_msgs_acc (f (Suc j)) a)\<close> set_ConsD)
+      then have "Process1b a m (f j) (f (Suc j))"
+        by (metis AcceptorAction.elims(2) Process1bLearnerLoop.elims(2) \<open>AcceptorAction a (f j) (f (Suc j))\<close> \<open>\<forall>a. \<not> Process1bLearnerLoopDone a (f j) (f (Suc j))\<close> \<open>\<forall>ln. \<not> Process1bLearnerLoopStep a ln (f j) (f (Suc j))\<close> \<open>\<forall>m. \<not> Process1a a m (f j) (f (Suc j))\<close>)
+      then show "(\<exists>k. i \<le> k \<and> k < Suc j \<and> 
+              m \<notin> set (known_msgs_acc (f k) a)
+            \<and> Process1b a m (f k) (f (1 + k)))"
+        by (metis False \<open>i < Suc j\<close> less_Suc_eq less_Suc_eq_le plus_1_eq_Suc)
+    qed
+  qed
+qed
+
+fun step_1a_constraint_1 :: "Acceptor set \<Rightarrow> Ballot \<Rightarrow> State \<Rightarrow> bool" where
+  "step_1a_constraint_1 Q b st = (\<forall>a \<in> Q. \<forall> mb :: Ballot. MaxBal st a mb \<longrightarrow> mb \<le> b)"
+fun step_1a_constraint_2 :: "Acceptor \<Rightarrow> State \<Rightarrow> bool" where
+  "step_1a_constraint_2 a st = (queued_msg st a = None)"
+fun step_1a_constraint_3 :: "Acceptor \<Rightarrow> State \<Rightarrow> bool" where
+  "step_1a_constraint_3 a st = (\<not> two_a_lrn_loop st a)"
+fun step_1a_constraint_4 :: "Acceptor set \<Rightarrow> Ballot \<Rightarrow> State \<Rightarrow> bool" where
+  "step_1a_constraint_4 Q b st = 
+    (\<forall>a \<in> Q. \<not> (\<exists>M \<in> set (msgs st). M \<noteq> M1a b \<and> Recv_acc st a M \<and> type M = T1a))"
+fun step_1a_constraint_5 :: "Acceptor set \<Rightarrow> Ballot \<Rightarrow> State \<Rightarrow> bool" where
+  "step_1a_constraint_5 Q b st = 
+    (\<forall>a\<in>Q. (\<forall>M\<in>set (msgs st).
+      (type M = T1b \<or> type M = T2a) \<longrightarrow> (\<exists>mb. B M mb \<and> b \<ge> mb)))"
+fun step_1a_constraints :: "Acceptor \<Rightarrow> Acceptor set \<Rightarrow> Ballot \<Rightarrow> State \<Rightarrow> bool" where
+  "step_1a_constraints a Q b st = (
+      step_1a_constraint_1 Q b st \<and>
+      step_1a_constraint_2 a st \<and>
+      step_1a_constraint_3 a st \<and>
+      step_1a_constraint_4 Q b st \<and>
+      step_1a_constraint_5 Q b st
+    )"
+
 lemma step_1a_constraints:
   assumes "Spec f"
       and "M1a b \<in> set (msgs (f i))"
       and "is_safe a"
+      and "a \<in> Q"
       and "M1a b \<notin> set (known_msgs_acc (f i) a)"
-      and "\<not> (\<exists>M \<in> set (msgs (f i)). M \<noteq> M1a b \<and> Recv_acc (f i) a M \<and> (type M = T1a \<or> type M = T1b))"
-      and "\<forall> mb :: Ballot. MaxBal (f i) a mb \<longrightarrow> mb < b"
-      and "queued_msg (f i) a = None"
-      and "\<not> two_a_lrn_loop (f i) a"
+
+      and "step_1a_constraints a Q b (f i)"
+
     shows "i < j \<and> M1a b \<notin> set (known_msgs_acc (f j) a) \<and>
            (\<forall> k. i \<le> k \<and> k \<le> j \<longrightarrow> \<not> ProposerSendAction (f k) (f (1 + k))
-                                      \<and> \<not> FakeAcceptorAction (f k) (f (1 + k)))
-           \<longrightarrow>
-           (\<forall> k. i \<le> k \<and> k \<le> j \<longrightarrow> \<not> (\<exists>M \<in> set (msgs (f k)). M \<noteq> M1a b \<and> Recv_acc (f k) a M \<and> (type M = T1a \<or> type M = T1b))
-                                    \<and> (\<forall> mb :: Ballot. MaxBal (f k) a mb \<longrightarrow> mb < b)
-                                    \<and> queued_msg (f k) a = None
-                                    \<and> \<not> two_a_lrn_loop (f k) a)"
+                                  \<and> \<not> FakeAcceptorAction (f k) (f (1 + k))
+                                  \<and> (\<forall>a. a \<notin> Q \<longrightarrow> \<not> AcceptorAction a (f k) (f (1 + k))))
+           \<longrightarrow> (\<forall> k. i \<le> k \<and> k \<le> j \<longrightarrow> step_1a_constraints a Q b (f k))"
 proof (induction j)
   case 0
   then show ?case
     by fastforce
 next
   case (Suc j)
-  assume ih:"i < j \<and>
-         M1a b \<notin> set (known_msgs_acc (f j) a) \<and>
-         (\<forall>k. i \<le> k \<and> k \<le> j \<longrightarrow>
-              \<not> ProposerSendAction (f k) (f (1 + k)) \<and>
-              \<not> FakeAcceptorAction (f k) (f (1 + k))) \<longrightarrow>
-         (\<forall>k. i \<le> k \<and> k \<le> j \<longrightarrow>
-              \<not> (\<exists>M\<in>set (msgs (f k)).
-                     M \<noteq> M1a b \<and>
-                     Recv_acc (f k) a M \<and> (type M = T1a \<or> type M = T1b)) \<and>
-              (\<forall>mb. MaxBal (f k) a mb \<longrightarrow> mb < b)
-                                    \<and> queued_msg (f k) a = None
-                                    \<and> \<not> two_a_lrn_loop (f k) a)"
+  assume ih:"i < j \<and> M1a b \<notin> set (known_msgs_acc (f j) a) \<and>
+           (\<forall> k. i \<le> k \<and> k \<le> j \<longrightarrow> \<not> ProposerSendAction (f k) (f (1 + k))
+                                  \<and> \<not> FakeAcceptorAction (f k) (f (1 + k))
+                                  \<and> (\<forall>a. a \<notin> Q \<longrightarrow> \<not> AcceptorAction a (f k) (f (1 + k))))
+           \<longrightarrow> (\<forall> k. i \<le> k \<and> k \<le> j \<longrightarrow> step_1a_constraints a Q b (f k))"
   then show ?case
   proof (clarify)
     fix k
     assume "i < Suc j"
        and "M1a b \<notin> set (known_msgs_acc (f (Suc j)) a)"
-       and "\<forall>k. i \<le> k \<and> k \<le> Suc j \<longrightarrow>
-             \<not> ProposerSendAction (f k) (f (1 + k)) \<and>
-             \<not> FakeAcceptorAction (f k) (f (1 + k))"
+       and block: "\<forall>k. i \<le> k \<and> k \<le> Suc j \<longrightarrow>
+                     \<not> ProposerSendAction (f k) (f (1 + k)) \<and>
+                     \<not> FakeAcceptorAction (f k) (f (1 + k)) \<and>
+                     (\<forall>a. a \<notin> Q \<longrightarrow> \<not> AcceptorAction a (f k) (f (1 + k)))"
        and "i \<le> k"
        and "k \<le> Suc j"
     have "M1a b \<notin> set (known_msgs_acc (f j) a)"
       by (metis \<open>M1a b \<notin> set (known_msgs_acc (f (Suc j)) a)\<close> assms(1) known_msgs_acc_preserved le_add2 plus_1_eq_Suc)
-    have "(\<forall>k. i \<le> k \<and> k \<le> j \<longrightarrow>
-              \<not> ProposerSendAction (f k) (f (1 + k)) \<and>
-              \<not> FakeAcceptorAction (f k) (f (1 + k)))"
-      using \<open>\<forall>k. i \<le> k \<and> k \<le> Suc j \<longrightarrow> \<not> ProposerSendAction (f k) (f (1 + k)) \<and> \<not> FakeAcceptorAction (f k) (f (1 + k))\<close> le_Suc_eq by presburger
-    have ihu:"(\<forall>k. i \<le> k \<and> k \<le> j \<longrightarrow>
-              \<not> (\<exists>M\<in>set (msgs (f k)).
-                     M \<noteq> M1a b \<and>
-                     Recv_acc (f k) a M \<and> (type M = T1a \<or> type M = T1b)) \<and>
-              (\<forall>mb. MaxBal (f k) a mb \<longrightarrow> mb < b))"
-      by (metis \<open>M1a b \<notin> set (known_msgs_acc (f j) a)\<close> \<open>\<forall>k. i \<le> k \<and> k \<le> j \<longrightarrow> \<not> ProposerSendAction (f k) (f (1 + k)) \<and> \<not> FakeAcceptorAction (f k) (f (1 + k))\<close> \<open>i < Suc j\<close> antisym assms(5) assms(6) ih less_SucE)
-    show "\<not> (\<exists>M\<in>set (msgs (f k)).
-                    M \<noteq> M1a b \<and>
-                    Recv_acc (f k) a M \<and> (type M = T1a \<or> type M = T1b))
-               \<and> (\<forall>mb. MaxBal (f k) a mb \<longrightarrow> mb < b)
-                                    \<and> queued_msg (f k) a = None
-                                    \<and> \<not> two_a_lrn_loop (f k) a"
-    proof (cases "k \<noteq> Suc j")
+    have ihp: "(\<forall> k. i \<le> k \<and> k \<le> j \<longrightarrow> \<not> ProposerSendAction (f k) (f (1 + k))
+                                  \<and> \<not> FakeAcceptorAction (f k) (f (1 + k))
+                                  \<and> (\<forall>a. a \<notin> Q \<longrightarrow> \<not> AcceptorAction a (f k) (f (1 + k))))"
+      using \<open>i \<le> k\<close> \<open>k \<le> Suc j\<close> block le_Suc_eq by blast
+    show "step_1a_constraints a Q b (f k)"
+    proof (cases "i = k")
       case True
-      then show ?thesis 
-        using \<open>\<forall>k. i \<le> k \<and> k \<le> j \<longrightarrow> \<not> (\<exists>M\<in>set (msgs (f k)). M \<noteq> M1a b \<and> Recv_acc (f k) a M \<and> (type M = T1a \<or> type M = T1b)) \<and> (\<forall>mb. MaxBal (f k) a mb \<longrightarrow> mb < b)\<close> \<open>i \<le> k\<close> \<open>k \<le> Suc j\<close> le_SucE by blast
+      then show ?thesis
+        using \<open>step_1a_constraints a Q b (f i)\<close> by fastforce
     next
       case False
-      have ihu1: "\<not> (\<exists>M\<in>set (msgs (f j)).
-                     M \<noteq> M1a b \<and>
-                     Recv_acc (f j) a M \<and> (type M = T1a \<or> type M = T1b))"
-        using \<open>i < Suc j\<close> ihu less_Suc_eq_le by blast
-      have ihu2: "(\<forall>mb. MaxBal (f j) a mb \<longrightarrow> mb < b)"
-        using \<open>i < Suc j\<close> ihu less_Suc_eq_le by blast
-      have r1: "known_msgs_acc (f j) a = known_msgs_acc (f (Suc j)) a \<longrightarrow> (\<forall>mb. MaxBal (f k) a mb \<longrightarrow> mb < b)"
-        using False MaxBal.simps ihu2 by presburger
-      have r2: "known_msgs_acc (f j) a = known_msgs_acc (f (Suc j)) a \<and> set (msgs (f j)) = set (msgs (f (Suc j))) 
-            \<longrightarrow> \<not> (\<exists>M\<in>set (msgs (f k)). M \<noteq> M1a b \<and> Recv_acc (f k) a M \<and> (type M = T1a \<or> type M = T1b))"
-        unfolding Recv_acc.simps Proper_acc.simps
-        by (metis False Proper_acc.elims(1) Recv_acc.elims(3) Wellformed_Constant assms(1) ihu1)
-      have r3: "queued_msg (f j) a = queued_msg (f (Suc j)) a \<longrightarrow> queued_msg (f k) a = None"
-        by (metis False MessageType.distinct(1) QueuedMsgResult QueuedMsgSpec1.elims(2) QueuedMsgSpec2.elims(2) QueuedMsgSpec2_Conserved assms(1) assms(3) ihu1 type.simps(1))
-      have r4: "two_a_lrn_loop (f j) a = two_a_lrn_loop (f (Suc j)) a \<longrightarrow> \<not> two_a_lrn_loop (f k) a "
-        by (metis False Orderings.order_eq_iff \<open>M1a b \<notin> set (known_msgs_acc (f j) a)\<close> \<open>\<forall>k. i \<le> k \<and> k \<le> j \<longrightarrow> \<not> ProposerSendAction (f k) (f (1 + k)) \<and> \<not> FakeAcceptorAction (f k) (f (1 + k))\<close> \<open>i < Suc j\<close> assms(8) ih not_less_less_Suc_eq order_less_imp_le)
+      have "i < k"
+        by (simp add: False \<open>i \<le> k\<close> nat_less_le)
+      then have ihu: "step_1a_constraints a Q b (f j)"
+        by (metis \<open>M1a b \<notin> set (known_msgs_acc (f j) a)\<close> \<open>i < Suc j\<close> assms(6) ih ihp less_Suc_eq less_or_eq_imp_le)
+      then show ?thesis
+      proof (cases "k \<noteq> Suc j")
+        case True
+        then show ?thesis
+          by (metis False \<open>M1a b \<notin> set (known_msgs_acc (f j) a)\<close> \<open>i < Suc j\<close> \<open>i \<le> k\<close> \<open>k \<le> Suc j\<close> antisym ih ihp le_SucE less_antisym)
+      next
+        case False
+        then have "k = Suc j"
+          by simp
+        have ihu1: "step_1a_constraint_1 Q b (f j)"
+          using ihu step_1a_constraints.simps by blast
+        have ihu2: "step_1a_constraint_2 a (f j)"
+          using ihu step_1a_constraints.simps by blast
+        have ihu3: "step_1a_constraint_3 a (f j)"
+          using ihu step_1a_constraints.simps by blast
+        have ihu4: "step_1a_constraint_4 Q b (f j)"
+          using ihu step_1a_constraints.simps by blast
+        have ihu5: "step_1a_constraint_5 Q b (f j)"
+          using ihu step_1a_constraints.simps by blast
+
+        have r1: "\<forall>a \<in> Q. known_msgs_acc (f j) a = known_msgs_acc (f (Suc j)) a \<longrightarrow> (\<forall> mb :: Ballot. MaxBal (f k) a mb \<longrightarrow> mb \<le> b)"
+          using ihu1 False by auto
+        have r2: "queued_msg (f j) a = queued_msg (f (Suc j)) a \<longrightarrow> step_1a_constraint_2 a (f k)"
+          using ihu2 False by auto
+        have r3: "two_a_lrn_loop (f j) a = two_a_lrn_loop (f (Suc j)) a \<longrightarrow> step_1a_constraint_3 a (f k)"
+          using ihu3 False by auto
+        have r4: "(\<forall>m \<in> set (msgs (f (Suc j))). type m = T1a \<longrightarrow> m \<in> set (msgs (f j))) \<longrightarrow> step_1a_constraint_4 Q b (f k)"
+          unfolding step_1a_constraint_4.simps
+        proof (clarify)
+          fix a M
+          assume "\<forall>m\<in>set (msgs (f (Suc j))). type m = T1a \<longrightarrow> m \<in> set (msgs (f j))"
+             and "a \<in> Q"
+             and "M \<in> set (msgs (f k))"
+             and "M \<noteq> M1a b"
+             and "Recv_acc (f k) a M"
+             and "type M = T1a"
+          then show False
+          proof (cases "M \<notin> set (known_msgs_acc (f k) a)")
+            case True
+            then have "M \<notin> set (known_msgs_acc (f j) a)"
+              by (metis False assms(1) known_msgs_acc_preserved le_add2 plus_1_eq_Suc)
+            then have "Recv_acc (f j) a M"
+              by (metis MessageType.distinct(1) MessageType.distinct(3) Proper_acc.elims(1) Recv_acc.elims(2) Recv_acc.elims(3) Wellformed_Constant \<open>Recv_acc (f k) a M\<close> \<open>type M = T1a\<close> assms(1) empty_iff ref.simps(1) type.elims)
+            then show ?thesis
+              using False \<open>M \<in> set (msgs (f k))\<close> \<open>M \<noteq> M1a b\<close> \<open>\<forall>m\<in>set (msgs (f (Suc j))). type m = T1a \<longrightarrow> m \<in> set (msgs (f j))\<close> \<open>a \<in> Q\<close> \<open>type M = T1a\<close> ihu4 step_1a_constraint_4.simps by blast
+          next
+            case False
+            then show ?thesis
+              using Recv_acc.elims(2) \<open>Recv_acc (f k) a M\<close> by blast
+          qed
+        qed
+        have r5: "msgs (f (Suc j)) = msgs (f j) \<and> (\<forall>a \<in> Q. known_msgs_acc (f j) a = known_msgs_acc (f (Suc j)) a) \<longrightarrow> step_1a_constraint_5 Q b (f k)"
+          using ihu5
+          unfolding step_1a_constraint_5.simps
+          by (smt (verit) False MaxBal.simps Proper_acc.elims(1) Recv_acc.simps Wellformed_Constant assms(1))
       show ?thesis
       proof (cases "f j = f (Suc j)")
         case True
         then show ?thesis
-          by (metis False \<open>M1a b \<notin> set (known_msgs_acc (f j) a)\<close> \<open>\<forall>k. i \<le> k \<and> k \<le> j \<longrightarrow> \<not> ProposerSendAction (f k) (f (1 + k)) \<and> \<not> FakeAcceptorAction (f k) (f (1 + k))\<close> \<open>i < Suc j\<close> assms(7) assms(8) dual_order.eq_iff dual_order.strict_implies_order ih not_less_less_Suc_eq r1 r2)
+          using False ihu by presburger
       next
         case False
         have "Next (f j) (f (Suc j))"
           using False Spec.simps assms(1) by blast
         have "\<not> (ProposerSendAction (f j) (f (Suc j)))"
-          by (metis \<open>\<forall>k. i \<le> k \<and> k \<le> Suc j \<longrightarrow> \<not> ProposerSendAction (f k) (f (1 + k)) \<and> \<not> FakeAcceptorAction (f k) (f (1 + k))\<close> \<open>i < Suc j\<close> le_add2 less_Suc_eq_le plus_1_eq_Suc)
+          by (metis Suc_eq_plus1_left \<open>i < Suc j\<close> ihp le_refl less_Suc_eq_le)
         have "\<not> (FakeAcceptorAction (f j) (f (Suc j)))"
-          by (metis \<open>\<forall>k. i \<le> k \<and> k \<le> Suc j \<longrightarrow> \<not> ProposerSendAction (f k) (f (1 + k)) \<and> \<not> FakeAcceptorAction (f k) (f (1 + k))\<close> \<open>i < Suc j\<close> le_add2 less_Suc_eq_le plus_1_eq_Suc)
+          by (metis Suc_eq_plus1_left \<open>i < Suc j\<close> ihp le_refl less_Suc_eq_le)
         have "\<forall>m \<in> set (msgs (f j)). \<not> (Process1a a m (f j) (f (Suc j)))"
-          by (metis Process1a.elims(2) Process1a_Req_known_msgs \<open>M1a b \<notin> set (known_msgs_acc (f (Suc j)) a)\<close> assms(1) diff_Suc_1 ihu1)
-        have "\<forall>m \<in> set (msgs (f j)). \<not> (Process1b a m (f j) (f (Suc j)))"
-          by (metis Enabled.simps MessageType.distinct(1) Process1b_Enabled ihu1 type.simps(1))
+          by (metis Process1a.elims(2) Process1a_Req_known_msgs \<open>M1a b \<notin> set (known_msgs_acc (f (Suc j)) a)\<close> assms(1) assms(4) diff_Suc_1 ihu4 step_1a_constraint_4.elims(2))
+        have "\<forall>a. a \<notin> Q \<longrightarrow> (\<forall>m. \<not> (Process1a a m (f j) (f (Suc j))))"
+          by (metis Process1a_Next_Implies_AcceptorAction \<open>Next (f j) (f (Suc j))\<close> \<open>i < Suc j\<close> block le_add2 less_Suc_eq_le plus_1_eq_Suc)
+        have "\<forall>a. a \<notin> Q \<longrightarrow> (\<forall>m. \<not> (Process1b a m (f j) (f (Suc j))))"
+          by (metis Process1b_Next_Implies_AcceptorAction \<open>Next (f j) (f (Suc j))\<close> \<open>i < Suc j\<close> block le_add2 less_Suc_eq_le plus_1_eq_Suc)
         then show ?thesis
         proof (cases "LearnerProcessAction (f j) (f (Suc j))")
           case True
@@ -319,52 +365,52 @@ next
             assume "(\<exists>m\<in>set (msgs (f j)). LearnerRecv ln m (f j) (f (Suc j))) \<or>
                     (\<exists>blt val. LearnerDecide ln blt val (f j) (f (Suc j)))"
             then show ?thesis
-              unfolding LearnerRecv.simps LearnerDecide.simps
-            proof -
-              assume a1: "(\<exists>m\<in>set (msgs (f j)). Recv_lrn (f j) ln m \<and> f (Suc j) = f j \<lparr>known_msgs_lrn := \<lambda>x. if ln = x then m # known_msgs_lrn (f j) x else known_msgs_lrn (f j) x\<rparr>) \<or> (\<exists>blt val. ChosenIn (f j) ln blt val \<and> f (Suc j) = f j \<lparr>decision := \<lambda>x y. if x = ln \<and> y = blt then {val} \<union> decision (f j) x y else decision (f j) x y\<rparr>)"
-              have "i < j \<and> M1a b \<notin> set (known_msgs_acc (f j) a) \<and> (\<forall>n. i \<le> n \<and> n \<le> j \<longrightarrow> \<not> ProposerSendAction (f n) (f (1 + n)) \<and> \<not> FakeAcceptorAction (f n) (f (1 + n))) \<longrightarrow> (\<forall>n. i \<le> n \<and> n \<le> j \<longrightarrow> (\<forall>p. p \<notin> set (msgs (f n)) \<or> p = M1a b \<or> \<not> Recv_acc (f n) a p \<or> type p \<noteq> T1a \<and> type p \<noteq> T1b) \<and> (\<forall>na. MaxBal (f n) a na \<longrightarrow> na < b) \<and> queued_msg (f n) a = None \<and> \<not> two_a_lrn_loop (f n) a)"
-                using ih by blast
-              then have f2: "\<not> i < j \<or> (\<forall>n. \<not> i \<le> n \<or> \<not> n \<le> j \<or> (\<forall>p. p \<notin> set (msgs (f n)) \<or> p = M1a b \<or> \<not> Recv_acc (f n) a p \<or> type p \<noteq> T1a \<and> type p \<noteq> T1b) \<and> (\<forall>na. \<not> MaxBal (f n) a na \<or> na < b) \<and> queued_msg (f n) a = None \<and> \<not> two_a_lrn_loop (f n) a)"
-                using \<open>M1a b \<notin> set (known_msgs_acc (f j) a)\<close> \<open>\<forall>k. i \<le> k \<and> k \<le> j \<longrightarrow> \<not> ProposerSendAction (f k) (f (1 + k)) \<and> \<not> FakeAcceptorAction (f k) (f (1 + k))\<close> by presburger
-              have f3: "\<forall>n na. n < na \<or> \<not> n < Suc na \<or> na = n"
-                using less_antisym by blast
-              then have f4: "i < j \<or> j = i"
-                using \<open>i < Suc j\<close> by blast
-              have f5: "k < Suc j \<or> Suc j = k"
-                using f3 \<open>k \<le> Suc j\<close> less_Suc_eq_le by blast
-              obtain nn :: nat and pp :: PreMessage where
-                f6: "((\<exists>p. p \<in> set (msgs (f k)) \<and> p \<noteq> M1a b \<and> Recv_acc (f k) a p \<and> (type p = T1a \<or> type p = T1b)) \<or> (\<exists>n. MaxBal (f k) a n \<and> \<not> n < b) \<or> queued_msg (f k) a \<noteq> None \<or> two_a_lrn_loop (f k) a) = (pp \<in> set (msgs (f k)) \<and> pp \<noteq> M1a b \<and> Recv_acc (f k) a pp \<and> (type pp = T1a \<or> type pp = T1b) \<or> MaxBal (f k) a nn \<and> \<not> nn < b \<or> queued_msg (f k) a \<noteq> None \<or> two_a_lrn_loop (f k) a)"
-                by blast
-              have f7: "\<lparr>msgs = msgs (f j), known_msgs_acc = known_msgs_acc (f j), known_msgs_lrn = \<lambda>l. if ln = l then v0_2 # known_msgs_lrn (f j) l else known_msgs_lrn (f j) l, recent_msgs = recent_msgs (f j), queued_msg = queued_msg (f j), two_a_lrn_loop = two_a_lrn_loop (f j), processed_lrns = processed_lrns (f j), decision = decision (f j), BVal = BVal (f j), \<dots> = more (f j)\<rparr> = f j\<lparr>known_msgs_lrn := \<lambda>l. if ln = l then v0_2 # known_msgs_lrn (f j) l else known_msgs_lrn (f j) l\<rparr>"
-                by simp
-              obtain ppa :: PreMessage and nna :: nat and vv :: Value where
-                f8: "ppa \<in> set (msgs (f j)) \<and> Recv_lrn (f j) ln ppa \<and> f (Suc j) = f j \<lparr>known_msgs_lrn := \<lambda>l. if ln = l then ppa # known_msgs_lrn (f j) l else known_msgs_lrn (f j) l\<rparr> \<or> ChosenIn (f j) ln nna vv \<and> f (Suc j) = f j \<lparr>decision := \<lambda>l n. if l = ln \<and> n = nna then {vv} \<union> decision (f j) l n else decision (f j) l n\<rparr>"
-                using a1 by blast
-              have f9: "f (Suc j) = f j \<lparr>decision := \<lambda>l n. if l = ln \<and> n = nna then {vv} \<union> decision (f j) l n else decision (f j) l n\<rparr> \<longrightarrow> \<lparr>msgs = msgs (f j), known_msgs_acc = known_msgs_acc (f j), known_msgs_lrn = known_msgs_lrn (f j), recent_msgs = recent_msgs (f j), queued_msg = queued_msg (f j), two_a_lrn_loop = two_a_lrn_loop (f j), processed_lrns = processed_lrns (f j), decision = \<lambda>l n. if l = ln \<and> n = nna then {vv} \<union> decision (f j) l n else decision (f j) l n, BVal = BVal (f j), \<dots> = more (f j)\<rparr> = \<lparr>msgs = msgs (f (Suc j)), known_msgs_acc = known_msgs_acc (f (Suc j)), known_msgs_lrn = known_msgs_lrn (f (Suc j)), recent_msgs = recent_msgs (f (Suc j)), queued_msg = queued_msg (f (Suc j)), two_a_lrn_loop = two_a_lrn_loop (f (Suc j)), processed_lrns = processed_lrns (f (Suc j)), decision = decision (f (Suc j)), BVal = BVal (f (Suc j)), \<dots> = more (f (Suc j))\<rparr>"
-                by simp
-              have f10: "\<forall>ps f fa fb fc p fd fe ff u psa fg fh fi fj pa fk fl fm ua. (\<lparr>msgs = ps, known_msgs_acc = f, known_msgs_lrn = fa, recent_msgs = fb, queued_msg = fc, two_a_lrn_loop = p, processed_lrns = fd, decision = fe, BVal = ff, \<dots> = u::unit\<rparr> = \<lparr>msgs = psa, known_msgs_acc = fg, known_msgs_lrn = fh, recent_msgs = fi, queued_msg = fj, two_a_lrn_loop = pa, processed_lrns = fk, decision = fl, BVal = fm, \<dots> = ua\<rparr>) = (ps = psa \<and> f = fg \<and> fa = fh \<and> fb = fi \<and> fc = fj \<and> p = pa \<and> fd = fk \<and> fe = fl \<and> ff = fm \<and> u = ua)"
-                by simp
-              have f11: "i \<le> j"
-                using \<open>i < Suc j\<close> by auto
-              have f12: "queued_msg (f j) = queued_msg (f (Suc j)) \<and> queued_msg (f k) a \<noteq> None \<longrightarrow> queued_msg (f k) a = None"
-                using f4 f3 f2 by (metis (no_types) \<open>i \<le> k\<close> \<open>k \<le> Suc j\<close> assms(7) less_Suc_eq_le linorder_not_less)
-              moreover
-              { assume "ppa \<notin> set (msgs (f j)) \<or> \<not> Recv_lrn (f j) ln ppa \<or> f (Suc j) \<noteq> f j \<lparr>known_msgs_lrn := \<lambda>l. if ln = l then ppa # known_msgs_lrn (f j) l else known_msgs_lrn (f j) l\<rparr>"
-                moreover
-                { assume "(msgs (f j) = msgs (f (Suc j)) \<and> known_msgs_acc (f j) = known_msgs_acc (f (Suc j)) \<and> known_msgs_lrn (f j) = known_msgs_lrn (f (Suc j)) \<and> recent_msgs (f j) = recent_msgs (f (Suc j)) \<and> queued_msg (f j) = queued_msg (f (Suc j)) \<and> two_a_lrn_loop (f j) = two_a_lrn_loop (f (Suc j)) \<and> processed_lrns (f j) = processed_lrns (f (Suc j)) \<and> (\<lambda>l n. if l = ln \<and> n = nna then {vv} \<union> decision (f j) l n else decision (f j) l n) = decision (f (Suc j)) \<and> BVal (f j) = BVal (f (Suc j)) \<and> more (f j) = more (f (Suc j))) \<and> \<not> two_a_lrn_loop (f (Suc j)) a"
-                  then have "(msgs (f j) = msgs (f (Suc j)) \<and> known_msgs_acc (f j) = known_msgs_acc (f (Suc j)) \<and> known_msgs_lrn (f j) = known_msgs_lrn (f (Suc j)) \<and> recent_msgs (f j) = recent_msgs (f (Suc j)) \<and> queued_msg (f j) = queued_msg (f (Suc j)) \<and> two_a_lrn_loop (f j) = two_a_lrn_loop (f (Suc j)) \<and> processed_lrns (f j) = processed_lrns (f (Suc j)) \<and> (\<lambda>l n. if l = ln \<and> n = nna then {vv} \<union> decision (f j) l n else decision (f j) l n) = decision (f (Suc j)) \<and> BVal (f j) = BVal (f (Suc j)) \<and> more (f j) = more (f (Suc j))) \<and> Suc j \<noteq> k \<or> (msgs (f j) = msgs (f (Suc j)) \<and> known_msgs_acc (f j) = known_msgs_acc (f (Suc j)) \<and> known_msgs_lrn (f j) = known_msgs_lrn (f (Suc j)) \<and> recent_msgs (f j) = recent_msgs (f (Suc j)) \<and> queued_msg (f j) = queued_msg (f (Suc j)) \<and> two_a_lrn_loop (f j) = two_a_lrn_loop (f (Suc j)) \<and> processed_lrns (f j) = processed_lrns (f (Suc j)) \<and> (\<lambda>l n. if l = ln \<and> n = nna then {vv} \<union> decision (f j) l n else decision (f j) l n) = decision (f (Suc j)) \<and> BVal (f j) = BVal (f (Suc j)) \<and> more (f j) = more (f (Suc j))) \<and> \<not> two_a_lrn_loop (f k) a"
-                    by meson }
-                moreover
-                { assume "(msgs (f j) = msgs (f (Suc j)) \<and> known_msgs_acc (f j) = known_msgs_acc (f (Suc j)) \<and> known_msgs_lrn (f j) = known_msgs_lrn (f (Suc j)) \<and> recent_msgs (f j) = recent_msgs (f (Suc j)) \<and> queued_msg (f j) = queued_msg (f (Suc j)) \<and> two_a_lrn_loop (f j) = two_a_lrn_loop (f (Suc j)) \<and> processed_lrns (f j) = processed_lrns (f (Suc j)) \<and> (\<lambda>l n. if l = ln \<and> n = nna then {vv} \<union> decision (f j) l n else decision (f j) l n) = decision (f (Suc j)) \<and> BVal (f j) = BVal (f (Suc j)) \<and> more (f j) = more (f (Suc j))) \<and> \<not> j \<le> j"
-                  then have "(msgs (f j) = msgs (f (Suc j)) \<and> known_msgs_acc (f j) = known_msgs_acc (f (Suc j)) \<and> known_msgs_lrn (f j) = known_msgs_lrn (f (Suc j)) \<and> recent_msgs (f j) = recent_msgs (f (Suc j)) \<and> queued_msg (f j) = queued_msg (f (Suc j)) \<and> two_a_lrn_loop (f j) = two_a_lrn_loop (f (Suc j)) \<and> processed_lrns (f j) = processed_lrns (f (Suc j)) \<and> (\<lambda>l n. if l = ln \<and> n = nna then {vv} \<union> decision (f j) l n else decision (f j) l n) = decision (f (Suc j)) \<and> BVal (f j) = BVal (f (Suc j)) \<and> more (f j) = more (f (Suc j))) \<and> Suc j \<noteq> k \<or> (msgs (f j) = msgs (f (Suc j)) \<and> known_msgs_acc (f j) = known_msgs_acc (f (Suc j)) \<and> known_msgs_lrn (f j) = known_msgs_lrn (f (Suc j)) \<and> recent_msgs (f j) = recent_msgs (f (Suc j)) \<and> queued_msg (f j) = queued_msg (f (Suc j)) \<and> two_a_lrn_loop (f j) = two_a_lrn_loop (f (Suc j)) \<and> processed_lrns (f j) = processed_lrns (f (Suc j)) \<and> (\<lambda>l n. if l = ln \<and> n = nna then {vv} \<union> decision (f j) l n else decision (f j) l n) = decision (f (Suc j)) \<and> BVal (f j) = BVal (f (Suc j)) \<and> more (f j) = more (f (Suc j))) \<and> k \<le> j"
-                    by force }
-                ultimately have "(msgs (f j) = msgs (f (Suc j)) \<and> known_msgs_acc (f j) = known_msgs_acc (f (Suc j)) \<and> known_msgs_lrn (f j) = known_msgs_lrn (f (Suc j)) \<and> recent_msgs (f j) = recent_msgs (f (Suc j)) \<and> queued_msg (f j) = queued_msg (f (Suc j)) \<and> two_a_lrn_loop (f j) = two_a_lrn_loop (f (Suc j)) \<and> processed_lrns (f j) = processed_lrns (f (Suc j)) \<and> (\<lambda>l n. if l = ln \<and> n = nna then {vv} \<union> decision (f j) l n else decision (f j) l n) = decision (f (Suc j)) \<and> BVal (f j) = BVal (f (Suc j)) \<and> more (f j) = more (f (Suc j))) \<and> Suc j \<noteq> k \<or> (msgs (f j) = msgs (f (Suc j)) \<and> known_msgs_acc (f j) = known_msgs_acc (f (Suc j)) \<and> known_msgs_lrn (f j) = known_msgs_lrn (f (Suc j)) \<and> recent_msgs (f j) = recent_msgs (f (Suc j)) \<and> queued_msg (f j) = queued_msg (f (Suc j)) \<and> two_a_lrn_loop (f j) = two_a_lrn_loop (f (Suc j)) \<and> processed_lrns (f j) = processed_lrns (f (Suc j)) \<and> (\<lambda>l n. if l = ln \<and> n = nna then {vv} \<union> decision (f j) l n else decision (f j) l n) = decision (f (Suc j)) \<and> BVal (f j) = BVal (f (Suc j)) \<and> more (f j) = more (f (Suc j))) \<and> k \<le> j \<or> (msgs (f j) = msgs (f (Suc j)) \<and> known_msgs_acc (f j) = known_msgs_acc (f (Suc j)) \<and> known_msgs_lrn (f j) = known_msgs_lrn (f (Suc j)) \<and> recent_msgs (f j) = recent_msgs (f (Suc j)) \<and> queued_msg (f j) = queued_msg (f (Suc j)) \<and> two_a_lrn_loop (f j) = two_a_lrn_loop (f (Suc j)) \<and> processed_lrns (f j) = processed_lrns (f (Suc j)) \<and> (\<lambda>l n. if l = ln \<and> n = nna then {vv} \<union> decision (f j) l n else decision (f j) l n) = decision (f (Suc j)) \<and> BVal (f j) = BVal (f (Suc j)) \<and> more (f j) = more (f (Suc j))) \<and> j = i \<or> (msgs (f j) = msgs (f (Suc j)) \<and> known_msgs_acc (f j) = known_msgs_acc (f (Suc j)) \<and> known_msgs_lrn (f j) = known_msgs_lrn (f (Suc j)) \<and> recent_msgs (f j) = recent_msgs (f (Suc j)) \<and> queued_msg (f j) = queued_msg (f (Suc j)) \<and> two_a_lrn_loop (f j) = two_a_lrn_loop (f (Suc j)) \<and> processed_lrns (f j) = processed_lrns (f (Suc j)) \<and> (\<lambda>l n. if l = ln \<and> n = nna then {vv} \<union> decision (f j) l n else decision (f j) l n) = decision (f (Suc j)) \<and> BVal (f j) = BVal (f (Suc j)) \<and> more (f j) = more (f (Suc j))) \<and> \<not> two_a_lrn_loop (f k) a"
-                  using f11 f10 f9 f8 f4 f2 by (smt (z3))
-                then have "(pp \<notin> set (msgs (f k)) \<or> pp = M1a b \<or> \<not> Recv_acc (f k) a pp \<or> type pp \<noteq> T1a \<and> type pp \<noteq> T1b) \<and> (\<not> MaxBal (f k) a nn \<or> nn < b) \<and> queued_msg (f k) a = None \<and> \<not> two_a_lrn_loop (f k) a"
-                  using f12 f5 f4 f3 f2 by (smt (z3) \<open>i \<le> k\<close> assms(8) less_Suc_eq_le linorder_not_less r1 r2) }
-              ultimately show ?thesis
-                using f10 f7 f6 f5 f4 f3 f2
-                by (smt (z3) \<open>i \<le> k\<close> assms(8) less_Suc_eq_le linorder_not_less r1 r2 surjective update_convs(3))
+            proof (elim disjE)
+              assume "\<exists>m\<in>set (msgs (f j)). LearnerRecv ln m (f j) (f (Suc j))"
+              have "msgs (f j) = msgs (f (Suc j))"
+                using \<open>\<exists>m\<in>set (msgs (f j)). LearnerRecv ln m (f j) (f (Suc j))\<close> by fastforce
+              have "\<forall>a \<in> Q. known_msgs_acc (f j) a = known_msgs_acc (f (Suc j)) a"
+                by (metis (no_types, lifting) LearnerRecv.elims(2) \<open>\<exists>m\<in>set (msgs (f j)). LearnerRecv ln m (f j) (f (Suc j))\<close> ext_inject surjective update_convs(3))
+              have "step_1a_constraint_1 Q b (f k)"
+                unfolding step_1a_constraint_1.simps
+                using \<open>\<forall>a\<in>Q. known_msgs_acc (f j) a = known_msgs_acc (f (Suc j)) a\<close> r1 by blast
+              have "step_1a_constraint_2 a (f k)"
+                unfolding step_1a_constraint_2.simps
+                by (smt (verit, best) LearnerRecv.elims(2) \<open>\<exists>m\<in>set (msgs (f j)). LearnerRecv ln m (f j) (f (Suc j))\<close> ext_inject r2 step_1a_constraint_2.elims(2) surjective update_convs(3))
+              have "step_1a_constraint_3 a (f k)"
+                unfolding step_1a_constraint_3.simps
+                by (metis (no_types, lifting) LearnerRecv.elims(2) \<open>\<exists>m\<in>set (msgs (f j)). LearnerRecv ln m (f j) (f (Suc j))\<close> ext_inject r3 step_1a_constraint_3.elims(1) surjective update_convs(3))
+              have "step_1a_constraint_4 Q b (f k)"
+                unfolding step_1a_constraint_4.simps
+                by (metis \<open>msgs (f j) = msgs (f (Suc j))\<close> r4 step_1a_constraint_4.elims(2))
+              have "step_1a_constraint_5 Q b (f k)"
+                unfolding step_1a_constraint_5.simps
+                by (metis \<open>\<forall>a\<in>Q. known_msgs_acc (f j) a = known_msgs_acc (f (Suc j)) a\<close> \<open>msgs (f j) = msgs (f (Suc j))\<close> r5 step_1a_constraint_5.elims(2))
+              then show ?thesis
+                using \<open>step_1a_constraint_1 Q b (f k)\<close> \<open>step_1a_constraint_2 a (f k)\<close> \<open>step_1a_constraint_3 a (f k)\<close> \<open>step_1a_constraint_4 Q b (f k)\<close> step_1a_constraints.simps by presburger
+            next
+              assume "\<exists>blt val. LearnerDecide ln blt val (f j) (f (Suc j))"
+              have "msgs (f j) = msgs (f (Suc j))"
+                using \<open>\<exists>blt val. LearnerDecide ln blt val (f j) (f (Suc j))\<close> by force
+              have "\<forall>a \<in> Q. known_msgs_acc (f j) a = known_msgs_acc (f (Suc j)) a"
+                using \<open>\<exists>blt val. LearnerDecide ln blt val (f j) (f (Suc j))\<close> by fastforce
+              have "step_1a_constraint_1 Q b (f k)"
+                unfolding step_1a_constraint_1.simps
+                using \<open>\<forall>a\<in>Q. known_msgs_acc (f j) a = known_msgs_acc (f (Suc j)) a\<close> r1 by blast
+              have "step_1a_constraint_2 a (f k)"
+                unfolding step_1a_constraint_2.simps
+                using \<open>\<exists>blt val. LearnerDecide ln blt val (f j) (f (Suc j))\<close> r2 by force
+              have "step_1a_constraint_3 a (f k)"
+                unfolding step_1a_constraint_3.simps
+                using \<open>\<exists>blt val. LearnerDecide ln blt val (f j) (f (Suc j))\<close> r3 by force
+              have "step_1a_constraint_4 Q b (f k)"
+                unfolding step_1a_constraint_4.simps
+                by (metis \<open>msgs (f j) = msgs (f (Suc j))\<close> r4 step_1a_constraint_4.elims(2))
+              have "step_1a_constraint_5 Q b (f k)"
+                unfolding step_1a_constraint_5.simps
+                by (metis \<open>\<forall>a\<in>Q. known_msgs_acc (f j) a = known_msgs_acc (f (Suc j)) a\<close> \<open>msgs (f j) = msgs (f (Suc j))\<close> r5 step_1a_constraint_5.elims(2))
+              then show ?thesis
+                using \<open>step_1a_constraint_1 Q b (f k)\<close> \<open>step_1a_constraint_2 a (f k)\<close> \<open>step_1a_constraint_3 a (f k)\<close> \<open>step_1a_constraint_4 Q b (f k)\<close> step_1a_constraints.simps by presburger
             qed
           qed
         next
@@ -375,18 +421,18 @@ next
                                     \<and> queued_msg (f j) A = None 
                                     \<and> (\<exists>m \<in> set (msgs (f j)). Process1a A m (f j) (f (Suc j)))) \<or>
                       (\<exists>A :: Acceptor. is_safe A
-                                    \<and> queued_msg (f j) A \<noteq> None 
-                                    \<and> Process1b A (the (queued_msg (f j) A)) (f j) (f (Suc j))) \<or>
-                      (\<exists>A :: Acceptor. is_safe A
                                     \<and> queued_msg (f j) A = None 
                                     \<and> (\<exists>m \<in> set (msgs (f j)). Process1b A m (f j) (f (Suc j)))) \<or>
+                      (\<exists>A :: Acceptor. is_safe A
+                                    \<and> queued_msg (f j) A \<noteq> None 
+                                    \<and> Process1b A (the (queued_msg (f j) A)) (f j) (f (Suc j))) \<or>
                       (\<exists>A :: Acceptor. is_safe A
                                     \<and> two_a_lrn_loop (f j) A 
                                     \<and> (\<exists>l :: Learner. Process1bLearnerLoopStep A l (f j) (f (Suc j)))) \<or>
                       (\<exists>A :: Acceptor. is_safe A
                                     \<and> two_a_lrn_loop (f j) A 
                                     \<and> Process1bLearnerLoopDone A (f j) (f (Suc j)))"
-            using Acceptor_split by presburger
+            using Acceptor_split by blast
           then show ?thesis
           proof (elim disjE)
             assume "\<exists>A. is_safe A \<and>
@@ -400,29 +446,95 @@ next
                  and "queued_msg (f j) A = None"
                  and "m \<in> set (msgs (f j))"
                  and "Process1a A m (f j) (f (Suc j))"
-              define new1b where "new1b = M1b A (m # recent_msgs (f j) A)"
-              then show ?thesis
-              proof (cases "WellFormed (f j) new1b")
-                case True
-                then show ?thesis sorry
-              next
-                case False
-                then show ?thesis sorry
+              have "type m = T1a"
+                by (meson Process1a.elims(2) \<open>Process1a A m (f j) (f (Suc j))\<close>)
+              then have "m = M1a b"
+                by (meson Process1a.elims(2) \<open>Process1a A m (f j) (f (Suc j))\<close> \<open>\<forall>a. a \<notin> Q \<longrightarrow> (\<forall>m. \<not> Process1a a m (f j) (f (Suc j)))\<close> \<open>m \<in> set (msgs (f j))\<close> ihu4 step_1a_constraint_4.elims(2))
+              have "A \<noteq> a"
+                using \<open>Process1a A m (f j) (f (Suc j))\<close> \<open>\<forall>m\<in>set (msgs (f j)). \<not> Process1a a m (f j) (f (Suc j))\<close> \<open>m \<in> set (msgs (f j))\<close> by fastforce
+              have "A \<in> Q"
+                using \<open>Process1a A m (f j) (f (Suc j))\<close> \<open>\<forall>a. a \<notin> Q \<longrightarrow> (\<forall>m. \<not> Process1a a m (f j) (f (Suc j)))\<close> by blast
+              have "\<forall>a. a \<noteq> A \<longrightarrow> known_msgs_acc (f j) a = known_msgs_acc (f (Suc j)) a"
+                by (metis Process1a.elims(2) Store_acc.elims(2) \<open>Process1a A m (f j) (f (Suc j))\<close>)
+              have "M1a b # known_msgs_acc (f j) A = known_msgs_acc (f (Suc j)) A"
+                by (metis Process1a.elims(2) Store_acc.elims(2) \<open>Process1a A m (f j) (f (Suc j))\<close> \<open>m = M1a b\<close>)
+              then have "M1a b # known_msgs_acc (f j) A = known_msgs_acc (f k) A"
+                using \<open>k = Suc j\<close> by fastforce
+              have "B (M1a b) b"
+                by simp
+              have "\<exists>m\<in>set (known_msgs_acc (f k) A). B m b"
+                by (metis \<open>B (M1a b) b\<close> \<open>M1a b # known_msgs_acc (f j) A = known_msgs_acc (f (Suc j)) A\<close> \<open>k = Suc j\<close> list.set_intros(1))
+              have "\<forall>b2. B (M1a b) b2 \<longrightarrow> b2 \<le> b"
+                unfolding B.simps Tran.simps
+                by fastforce
+              then have "\<forall>x\<in>set (known_msgs_acc (f k) A). \<forall>b2. B x b2 \<longrightarrow> b2 \<le> b"
+                using ihu1 
+                unfolding step_1a_constraint_1.simps
+                by (metis \<open>A \<in> Q\<close> \<open>M1a b # known_msgs_acc (f j) A = known_msgs_acc (f (Suc j)) A\<close> \<open>k = Suc j\<close> dual_order.trans maxbal_absence not_le_imp_less set_ConsD)
+              have "B (M1a b) b"
+                by simp
+              have "\<exists>m\<in>set (known_msgs_acc (f k) A). B m b"
+                by (metis \<open>B (M1a b) b\<close> \<open>M1a b # known_msgs_acc (f j) A = known_msgs_acc (f (Suc j)) A\<close> \<open>k = Suc j\<close> list.set_intros(1))
+              have "\<forall>b2. B (M1a b) b2 \<longrightarrow> b2 \<le> b"
+                unfolding B.simps Tran.simps
+                by fastforce
+              then have "\<forall>x\<in>set (known_msgs_acc (f k) A). \<forall>b2. B x b2 \<longrightarrow> b2 \<le> b"
+                using ihu1 
+                unfolding step_1a_constraint_1.simps
+                using \<open>\<forall>x\<in>set (known_msgs_acc (f k) A). \<forall>b2. B x b2 \<longrightarrow> b2 \<le> b\<close> by fastforce
+              have c1: "step_1a_constraint_1 Q b (f k)"
+                unfolding step_1a_constraint_1.simps
+              proof (clarify)
+                fix a mb
+                assume "a \<in> Q"
+                   and "MaxBal (f k) a mb"
+                then show "mb \<le> b"
+                proof (cases "a = A")
+                  case True
+                  then show ?thesis
+                    using MaxBal.simps \<open>MaxBal (f k) a mb\<close> \<open>\<forall>x\<in>set (known_msgs_acc (f k) A). \<forall>b2. B x b2 \<longrightarrow> b2 \<le> b\<close> by blast
+                next
+                  case False
+                  then show ?thesis
+                    using \<open>MaxBal (f k) a mb\<close> \<open>\<forall>a. a \<noteq> A \<longrightarrow> known_msgs_acc (f j) a = known_msgs_acc (f (Suc j)) a\<close> \<open>a \<in> Q\<close> r1 by blast
+                qed
               qed
-            qed
-          next
-            assume "\<exists>A. is_safe A \<and>
-                      queued_msg (f j) A \<noteq> None \<and>
-                      Process1b A (the (queued_msg (f j) A)) (f j) (f (Suc j))"
-            then show ?thesis
-            proof (clarify)
-              fix A y
-              assume "is_safe A"
-                 and "queued_msg (f j) A = Some y"
-                 and "Process1b A (the (queued_msg (f j) A)) (f j) (f (Suc j))"
-              then show ?thesis
-                unfolding Process1b.simps
-                sorry
+              have c2: "step_1a_constraint_2 a (f k)"
+                by (smt (verit) Process1a.elims(2) Process1a_Req_known_msgs Recv_acc.elims(2) \<open>A \<noteq> a\<close> \<open>\<exists>A. is_safe A \<and> queued_msg (f j) A = None \<and> (\<exists>m\<in>set (msgs (f j)). Process1a A m (f j) (f (Suc j)))\<close> \<open>\<forall>a. a \<noteq> A \<longrightarrow> known_msgs_acc (f j) a = known_msgs_acc (f (Suc j)) a\<close> \<open>k = Suc j\<close> add_diff_cancel_left' assms(1) ihu2 plus_1_eq_Suc step_1a_constraint_2.elims(2) step_1a_constraint_2.elims(3))
+              have c3: "step_1a_constraint_3 a (f k)"
+                by (metis Process1a.elims(2) \<open>Process1a A m (f j) (f (Suc j))\<close> r3)
+              have c4: "step_1a_constraint_4 Q b (f k)"
+                by (smt (verit) MessageType.distinct(1) MessageType.distinct(3) PreMessage.distinct(1) Process1a.elims(2) Send.elims(2) \<open>\<exists>A. is_safe A \<and> queued_msg (f j) A = None \<and> (\<exists>m\<in>set (msgs (f j)). Process1a A m (f j) (f (Suc j)))\<close> r4 set_ConsD type.elims)
+
+              have "(\<forall>ba. (\<forall>m \<in> set (recent_msgs (f j) A). B m ba \<longrightarrow> ba \<le> b))"
+                by (metis RecentMsgsSpec.elims(2) RecentMsgsSpecResult \<open>\<forall>x\<in>set (known_msgs_acc (f k) A). \<forall>b2. B x b2 \<longrightarrow> b2 \<le> b\<close> \<open>is_safe A\<close> \<open>k = Suc j\<close> assms(1) known_msgs_acc_preserved less_Suc_eq_le nless_le order_refl subsetD)
+              then have "(\<forall>ba. M1a ba \<in> \<Union> (set (map Tran (recent_msgs (f j) A))) \<longrightarrow> ba \<le> b)"
+                by (smt (verit, del_insts) B_1a KnownMsgs_accSpec.elims(2) KnownMsgs_accSpecResult RecentMsgsSpec.elims(2) RecentMsgsSpecResult \<open>M1a b # known_msgs_acc (f j) A = known_msgs_acc (f (Suc j)) A\<close> \<open>\<forall>x\<in>set (known_msgs_acc (f k) A). \<forall>b2. B x b2 \<longrightarrow> b2 \<le> b\<close> \<open>is_safe A\<close> \<open>k = Suc j\<close> assms(1) bal.simps(1) imageE in_mono list.set_map mem_simps(9) set_subset_Cons type.simps(1))
+              then have "B (M1b A (m # recent_msgs (f j) A)) b"
+                by (simp add: \<open>m = M1a b\<close>)
+
+              have c5: "step_1a_constraint_5 Q b (f k)"
+                unfolding step_1a_constraint_5.simps
+              proof (clarify)
+                fix a M
+                assume "a \<in> Q"
+                   and "M \<in> set (msgs (f k))"
+                   and "type M = T1b \<or> type M = T2a"
+                then show "\<exists>mb. B M mb \<and> mb \<le> b"
+                proof (cases "WellFormed (f j) (M1b A (m # recent_msgs (f j) A))")
+                  case True
+                  then show ?thesis
+                    by (smt (verit) Process1a.elims(2) Send.elims(2) \<open>B (M1a b) b\<close> \<open>B (M1b A (m # recent_msgs (f j) A)) b\<close> \<open>M \<in> set (msgs (f k))\<close> \<open>Process1a A m (f j) (f (Suc j))\<close> \<open>\<forall>b2. B (M1a b) b2 \<longrightarrow> b2 \<le> b\<close> \<open>a \<in> Q\<close> \<open>k = Suc j\<close> \<open>type M = T1b \<or> type M = T2a\<close> ihu5 set_ConsD step_1a_constraint_5.elims(2))
+                next
+                  case False
+                  have "M \<in> set (msgs (f j))"
+                    by (metis False Process1a.elims(2) \<open>M \<in> set (msgs (f k))\<close> \<open>Process1a A m (f j) (f (Suc j))\<close> \<open>k = Suc j\<close>)
+                  then show ?thesis
+                    by (meson \<open>a \<in> Q\<close> \<open>type M = T1b \<or> type M = T2a\<close> ihu5 step_1a_constraint_5.elims(2))
+                qed
+              qed
+              show ?thesis
+                using c1 c2 c3 c4 c5 step_1a_constraints.simps by presburger
             qed
           next
             assume "\<exists>A. is_safe A \<and>
@@ -435,10 +547,61 @@ next
                  and "queued_msg (f j) A = None"
                  and "m\<in>set (msgs (f j))"
                  and "Process1b A m (f j) (f (Suc j))"
+
+              have c2: "step_1a_constraint_2 a (f k)"
+                unfolding step_1a_constraint_2.simps
+                by (metis Process1b.elims(2) \<open>Process1b A m (f j) (f (Suc j))\<close> \<open>k = Suc j\<close> ihu2 step_1a_constraint_2.elims(2))
+              have c4: "step_1a_constraint_4 Q b (f k)"
+                by (smt (verit) Process1b.simps \<open>Process1b A m (f j) (f (Suc j))\<close> r4)
+
+              have "Recv_acc (f j) A m"
+                using Process1b.simps \<open>Process1b A m (f j) (f (Suc j))\<close> by blast
+              have "type m = T1b"
+                using Process1b.simps \<open>Process1b A m (f j) (f (Suc j))\<close> by blast
+              then have "\<forall> mb :: Ballot. B m mb \<longrightarrow> mb \<le> b"
+                using \<open>Recv_acc (f j) A m\<close> ihu5
+                sledgehammer
+
+              have c1: "step_1a_constraint_1 Q b (f k)"
+                unfolding step_1a_constraint_1.simps Process1b.simps
+                sorry
+              have c3: "step_1a_constraint_3 a (f k)"
+                unfolding step_1a_constraint_3.simps
+                sorry
+              have c5: "step_1a_constraint_5 Q b (f k)"
+                sorry
+
+              show ?thesis
+                using c1 c2 c3 c4 c5 step_1a_constraints.simps by presburger
+            qed
+          next
+            assume "\<exists>A. is_safe A \<and>
+                      queued_msg (f j) A \<noteq> None \<and>
+                      Process1b A (the (queued_msg (f j) A)) (f j) (f (Suc j))"
+            then show ?thesis
+            proof (clarify)
+              fix A y
+              assume "is_safe A"
+                 and "queued_msg (f j) A = Some y"
+                 and "Process1b A (the (queued_msg (f j) A)) (f j) (f (Suc j))"
               then have "A \<noteq> a"
+                by (metis ihu2 option.discI step_1a_constraint_2.elims(2))
+              have c1: "step_1a_constraint_1 Q b (f k)"
                 sorry
-              then show ?thesis
+              have "queued_msg (f j) a = queued_msg (f (Suc j)) a"
+                by (metis Process1b.elims(2) \<open>A \<noteq> a\<close> \<open>Process1b A (the (queued_msg (f j) A)) (f j) (f (Suc j))\<close>)
+              then have c2: "step_1a_constraint_2 a (f k)"
+                using r2 by fastforce
+              have "two_a_lrn_loop (f j) a = two_a_lrn_loop (f (Suc j)) a"
+                by (smt (verit) Process1b.elims(1) \<open>A \<noteq> a\<close> \<open>Process1b A (the (queued_msg (f j) A)) (f j) (f (Suc j))\<close>)
+              then have c3: "step_1a_constraint_3 a (f k)"
+                using r3 by fastforce
+              have c4: "step_1a_constraint_4 Q b (f k)"
                 sorry
+              have c5: "step_1a_constraint_5 Q b (f k)"
+                sorry
+              show ?thesis
+                using c1 c2 c3 c4 c5 step_1a_constraints.simps by presburger
             qed
           next
             assume "\<exists>A. is_safe A \<and>
@@ -451,9 +614,20 @@ next
                  and "two_a_lrn_loop (f j) A"
                  and "Process1bLearnerLoopStep A l (f j) (f (Suc j))"
               then have "A \<noteq> a"
+                using ihu3 step_1a_constraint_3.elims(1) by blast
+              have c1: "step_1a_constraint_1 Q b (f k)"
                 sorry
-              then show ?thesis
+              have c2: "step_1a_constraint_2 a (f k)"
                 sorry
+              have c3: "step_1a_constraint_3 a (f k)"
+                sorry
+              have c4: "step_1a_constraint_4 Q b (f k)"
+                sorry
+              have c5: "step_1a_constraint_5 Q b (f k)"
+                unfolding step_1a_constraint_5.simps
+                sorry
+              show ?thesis
+                using c1 c2 c3 c4 c5 step_1a_constraints.simps by presburger
             qed
           next
             assume "\<exists>A. is_safe A \<and>
@@ -466,191 +640,24 @@ next
                  and "two_a_lrn_loop (f j) A"
                  and "Process1bLearnerLoopDone A (f j) (f (Suc j))"
               then have "A \<noteq> a"
+                using ihu3 by fastforce
+              have c1: "step_1a_constraint_1 Q b (f k)"
                 sorry
-              then show ?thesis
+              have c2: "step_1a_constraint_2 a (f k)"
                 sorry
+              have c3: "step_1a_constraint_3 a (f k)"
+                sorry
+              have c4: "step_1a_constraint_4 Q b (f k)"
+                sorry
+              have c5: "step_1a_constraint_5 Q b (f k)"
+                sorry
+              show ?thesis
+                using c1 c2 c3 c4 c5 step_1a_constraints.simps by presburger
             qed
           qed
         qed
       qed
     qed
-  qed
-qed
-
-lemma step_1a_full:
-  assumes "Spec f"
-      and "M1a b \<in> set (msgs (f i))"
-      and "\<forall> mb :: Ballot. MaxBal (f i) a mb \<longrightarrow> mb < b"
-      and "is_safe a"
-      and "M1a b \<notin> set (known_msgs_acc (f i) a)"
-      and "\<not> (\<exists>M \<in> set (msgs (f i)). M \<noteq> M1a b \<and> Recv_acc (f i) a M \<and> (type M = T1a \<or> type M = T1b))"
-    shows "M1a b \<in> set (known_msgs_acc (f (i + j)) a) \<and>
-           (\<forall> k. i \<le> k \<and> k \<le> i + j \<longrightarrow> \<not> ProposerSendAction (f k) (f (1 + k))
-                                      \<and> \<not> FakeAcceptorAction (f k) (f (1 + k)))
-           \<longrightarrow>
-           (\<exists>k. i \<le> k \<and> k < i + j \<and>
-             (\<forall> mb :: Ballot. MaxBal (f k) a mb \<longrightarrow> mb < b) \<and>
-             \<not> (\<exists>M \<in> set (msgs (f k)). M \<noteq> M1a b \<and> Recv_acc (f k) a M \<and> (type M = T1a \<or> type M = T1b)))"
-proof (induction j)
-  case 0
-  then show ?case
-    by (metis assms(5) verit_sum_simplify)
-next
-  case (Suc j)
-  then show ?case sorry
-qed
-
-lemma step_:
-  assumes "Spec f"
-      and "M1a b \<in> set (msgs (f i))"
-      and "\<forall> mb :: Ballot. MaxBal (f i) a mb \<longrightarrow> mb < b"
-      and "is_safe a"
-      and "M1a b \<notin> set (known_msgs_acc (f i) a)"
-      and "\<not> (\<exists>M \<in> set (msgs (f i)). M \<noteq> M1a b \<and> Recv_acc (f i) a M \<and> (type M = T1a \<or> type M = T1b))"
-    shows "i < j \<and> M1a b \<in> set (known_msgs_acc (f j) a) \<and>
-           (\<forall> k. i < k \<and> k < j \<longrightarrow> \<not> ProposerSendAction (f k) (f (1 + k))
-                                 \<and> \<not> FakeAcceptorAction (f k) (f (1 + k)))
-           \<longrightarrow>
-           (\<exists>k. i \<le> k \<and> k < j \<and> 
-             M1a b \<notin> set (known_msgs_acc (f k) a) \<and>
-             Process1a a (M1a b) (f k) (f (1 + k)) \<and>
-             (\<forall> mb :: Ballot. MaxBal (f k) a mb \<longrightarrow> mb < b) \<and>
-             \<not> (\<exists>M \<in> set (msgs (f k)). M \<noteq> M1a b \<and> Recv_acc (f k) a M \<and> (type M = T1a \<or> type M = T1b)))"
-proof (induction j)
-  case 0
-  then show ?case 
-    by fastforce
-next
-  case (Suc j)
-  assume ih: "i < j \<and>
-         M1a b \<in> set (known_msgs_acc (f j) a) \<and>
-         (\<forall>k. i < k \<and> k < j \<longrightarrow>
-              \<not> ProposerSendAction (f k) (f (1 + k)) \<and>
-              \<not> FakeAcceptorAction (f k) (f (1 + k))) \<longrightarrow>
-         (\<exists>k\<ge>i. k < j \<and>
-                 M1a b \<notin> set (known_msgs_acc (f k) a) \<and>
-                 Process1a a (M1a b) (f k) (f (1 + k)) \<and>
-                 (\<forall>mb. MaxBal (f k) a mb \<longrightarrow> mb < b) \<and>
-                 \<not> (\<exists>M\<in>set (msgs (f k)).
-                        M \<noteq> M1a b \<and>
-                        Recv_acc (f k) a M \<and>
-                        (type M = T1a \<or> type M = T1b)))"
-  show ?case
-  proof (clarify)
-    assume "i < Suc j"
-       and "M1a b \<in> set (known_msgs_acc (f (Suc j)) a)"
-       and "\<forall>k. i < k \<and> k < Suc j \<longrightarrow>
-            \<not> ProposerSendAction (f k) (f (1 + k)) \<and>
-            \<not> FakeAcceptorAction (f k) (f (1 + k))"
-    then show "\<exists>k\<ge>i. k < Suc j \<and>
-           M1a b \<notin> set (known_msgs_acc (f k) a) \<and>
-           Process1a a (M1a b) (f k) (f (1 + k)) \<and>
-           (\<forall>mb. MaxBal (f k) a mb \<longrightarrow> mb < b) \<and>
-           \<not> (\<exists>M\<in>set (msgs (f k)).
-                  M \<noteq> M1a b \<and>
-                  Recv_acc (f k) a M \<and>
-                  (type M = T1a \<or> type M = T1b))"
-    proof (cases "i = j")
-      case True
-      then show ?thesis
-        by (metis \<open>M1a b \<in> set (known_msgs_acc (f (Suc j)) a)\<close> \<open>i < Suc j\<close> assms(1) assms(2) assms(3) assms(4) assms(5) assms(6) le_less_Suc_eq step_1a_only)
-    next
-      case False
-      have "i < j"
-        using False \<open>i < Suc j\<close> by linarith
-      have "(\<forall>k. i < k \<and> k < j \<longrightarrow>
-              \<not> ProposerSendAction (f k) (f (1 + k)) \<and>
-              \<not> FakeAcceptorAction (f k) (f (1 + k)))"
-        using \<open>\<forall>k. i < k \<and> k < Suc j \<longrightarrow> \<not> ProposerSendAction (f k) (f (1 + k)) \<and> \<not> FakeAcceptorAction (f k) (f (1 + k))\<close> less_Suc_eq by blast
-      then show ?thesis sorry
-    qed
-
-
-      proof (cases "M1a b \<in> set (known_msgs_acc (f j) a)")
-        case True
-        then show ?thesis
-          by (metis Suc \<open>\<forall>k. i < k \<and> k < Suc j \<longrightarrow> \<not> ProposerSendAction (f k) (f (1 + k)) \<and> \<not> FakeAcceptorAction (f k) (f (1 + k))\<close> \<open>i < Suc j\<close> assms(5) less_Suc_eq)
-      next
-        case False
-          have "Next (f j) (f (Suc j))"
-            by (metis False Spec.elims(2) \<open>M1a b \<in> set (known_msgs_acc (f (Suc j)) a)\<close> assms(1))
-          then have "\<not> (ProposerSendAction (f j) (f (Suc j)))"
-            by (metis False ProposerSendAction.elims(2) Send1a.elims(2) \<open>M1a b \<in> set (known_msgs_acc (f (Suc j)) a)\<close> ext_inject surjective update_convs(1))
-          have "\<forall> ln m. \<not> (LearnerRecv ln m (f j) (f (Suc j)))"
-            by (smt (verit, ccfv_SIG) False LearnerRecv.simps \<open>M1a b \<in> set (known_msgs_acc (f (Suc j)) a)\<close> ext_inject surjective update_convs(3))
-          have "\<forall> ln blt val. \<not> (LearnerDecide ln blt val (f j) (f (Suc j)))"
-            using False \<open>M1a b \<in> set (known_msgs_acc (f (Suc j)) a)\<close> by force
-          then have "\<forall>a. \<not> (LearnerProcessAction (f j) (f (Suc j)))"
-            by (meson LearnerAction.elims(2) LearnerProcessAction.elims(1) \<open>\<forall>ln m. \<not> LearnerRecv ln m (f j) (f (Suc j))\<close>)
-          have "\<forall>a. \<not> (FakeSend1b a (f j) (f (Suc j)))"
-            by (metis FakeSend1b.elims(1) False \<open>M1a b \<in> set (known_msgs_acc (f (Suc j)) a)\<close> ext_inject surjective update_convs(1))
-          have "\<forall>a. \<not> (FakeSend2a a (f j) (f (Suc j)))"
-            by (metis FakeSend2a.simps False \<open>M1a b \<in> set (known_msgs_acc (f (Suc j)) a)\<close> ext_inject surjective update_convs(1))
-          then have "\<not> (FakeAcceptorAction (f j) (f (Suc j)))"
-            using FakeAcceptorAction.simps \<open>\<forall>a. \<not> FakeSend1b a (f j) (f (Suc j))\<close> by presburger
-          then have "AcceptorProcessAction (f j) (f (Suc j))"
-            by (meson LearnerAction.elims(2) LearnerProcessAction.elims(2) Next.simps \<open>Next (f j) (f (Suc j))\<close> \<open>\<forall>ln blt val. \<not> LearnerDecide ln blt val (f j) (f (Suc j))\<close> \<open>\<forall>ln m. \<not> LearnerRecv ln m (f j) (f (Suc j))\<close> \<open>\<not> ProposerSendAction (f j) (f (Suc j))\<close>)
-          have "\<forall> A m. a \<noteq> A \<longrightarrow> \<not> (Process1a A m (f j) (f (Suc j)))"
-            by (metis False Process1a.elims(2) Store_acc.elims(2) \<open>M1a b \<in> set (known_msgs_acc (f (Suc j)) a)\<close>)
-          have "\<forall> A m. a \<noteq> A \<longrightarrow> \<not> (Process1b A m (f j) (f (Suc j)))"
-            by (metis False Process1b.elims(2) Store_acc.elims(2) \<open>M1a b \<in> set (known_msgs_acc (f (Suc j)) a)\<close>)
-          have "\<forall> a. \<not> (Process1bLearnerLoopDone a (f j) (f (Suc j)))"
-            using False \<open>M1a b \<in> set (known_msgs_acc (f (Suc j)) a)\<close> by force
-          have "\<forall> ln. \<not> (Process1bLearnerLoopStep a ln (f j) (f (Suc j)))"
-            unfolding Process1bLearnerLoopStep.simps
-            by (smt (verit, ccfv_SIG) False PreMessage.distinct(3) Store_acc.elims(2) \<open>M1a b \<in> set (known_msgs_acc (f (Suc j)) a)\<close> set_ConsD)  
-          then have "\<forall> A. a \<noteq> A \<longrightarrow> \<not> AcceptorAction A (f j) (f (Suc j))"
-          proof -
-            { fix aa :: Acceptor
-              have "known_msgs_acc (f (Suc j)) \<noteq> known_msgs_acc (f j) \<and> known_msgs_acc (f (Suc j)) a \<noteq> known_msgs_acc (f j) a"
-                using False \<open>M1a b \<in> set (known_msgs_acc (f (Suc j)) a)\<close> by fastforce
-              then have "aa = a \<or> \<not> AcceptorAction aa (f j) (f (Suc j))"
-                by (metis (full_types) AcceptorAction.elims(2) Process1bLearnerLoop.elims(2) Process1bLearnerLoopStep.elims(2) Store_acc.elims(2) \<open>\<forall>A m. a \<noteq> A \<longrightarrow> \<not> Process1a A m (f j) (f (Suc j))\<close> \<open>\<forall>A m. a \<noteq> A \<longrightarrow> \<not> Process1b A m (f j) (f (Suc j))\<close> \<open>\<forall>a. \<not> Process1bLearnerLoopDone a (f j) (f (Suc j))\<close>) }
-            then show ?thesis
-              by (metis (no_types))
-          qed
-          then have "AcceptorAction a (f j) (f (Suc j))"
-            by (metis AcceptorProcessAction.simps \<open>AcceptorProcessAction (f j) (f (Suc j))\<close>)
-          have "\<forall> m. (M1a b) \<noteq> m \<longrightarrow> \<not> (Process1a a m (f j) (f (Suc j)))"
-            unfolding Process1a.simps
-            by (metis False Store_acc.elims(2) \<open>M1a b \<in> set (known_msgs_acc (f (Suc j)) a)\<close> set_ConsD)
-          have "\<not> (Process1b a (M1a b) (f j) (f (Suc j)))"
-            by simp
-          have "\<forall> m. (M1a b) \<noteq> m \<longrightarrow> \<not> (Process1b a m (f j) (f (Suc j)))"
-            unfolding Process1b.simps
-            by (metis (no_types, lifting) False Store_acc.elims(2) \<open>M1a b \<in> set (known_msgs_acc (f (Suc j)) a)\<close> set_ConsD)
-          then have "\<forall> m. \<not> (Process1b a m (f j) (f (Suc j)))"
-            by (metis \<open>\<not> Process1b a (M1a b) (f j) (f (Suc j))\<close>)
-          then have "Process1a a (M1a b) (f j) (f (Suc j))"
-            by (metis AcceptorAction.elims(2) Process1bLearnerLoop.elims(2) \<open>AcceptorAction a (f j) (f (Suc j))\<close> \<open>\<forall>a. \<not> Process1bLearnerLoopDone a (f j) (f (Suc j))\<close> \<open>\<forall>ln. \<not> Process1bLearnerLoopStep a ln (f j) (f (Suc j))\<close> \<open>\<forall>m. M1a b \<noteq> m \<longrightarrow> \<not> Process1a a m (f j) (f (Suc j))\<close>)
-          then have "\<exists>k. i \<le> k \<and> k < Suc j \<and> Process1a a (M1a b) (f k) (f (1 + k))"
-            by (metis \<open>i < Suc j\<close> less_Suc_eq less_Suc_eq_le plus_1_eq_Suc)
-          have "\<forall>k. i < k \<and> k < j \<longrightarrow>
-              \<not> ProposerSendAction (f k) (f (1 + k)) \<and>
-              \<not> FakeAcceptorAction (f k) (f (1 + k))"
-            using \<open>\<forall>k. i < k \<and> k < Suc j \<longrightarrow> \<not> ProposerSendAction (f k) (f (1 + k)) \<and> \<not> FakeAcceptorAction (f k) (f (1 + k))\<close> less_Suc_eq by presburger
-          show ?thesis
-          proof (cases "i < j")
-            case True
-            have "\<exists>k\<ge>i. k < j \<and>
-                 Process1a a (M1a b) (f k) (f (1 + k)) \<and>
-                 (\<forall>mb. MaxBal (f k) a mb \<longrightarrow> mb < b) \<and>
-                 \<not> (\<exists>M\<in>set (msgs (f k)).
-                        M \<noteq> M1a b \<and>
-                        Recv_acc (f k) a M \<and>
-                        (type M = T1a \<or> type M = T1b))"
-              sorry
-            then show ?thesis sorry
-          next
-            case False
-            have "i = j"
-              using False \<open>i < Suc j\<close> less_Suc_eq by blast
-            then show ?thesis
-              using \<open>\<exists>k\<ge>i. k < Suc j \<and> Process1a a (M1a b) (f k) (f (1 + k))\<close> assms(3) assms(6) le_less_Suc_eq by blast
-          qed
-        qed
-      qed
-
   qed
 qed
 
@@ -1184,3 +1191,458 @@ theorem LivenessResult :
   sorry
 
 end
+
+
+
+
+
+
+
+
+
+
+
+(*
+lemma step_1a_constraints:
+  assumes "Spec f"
+      and "M1a b \<in> set (msgs (f i))"
+      and "is_safe a"
+      and "M1a b \<notin> set (known_msgs_acc (f i) a)"
+      and "\<not> (\<exists>M \<in> set (msgs (f i)). M \<noteq> M1a b \<and> Recv_acc (f i) a M \<and> (type M = T1a \<or> type M = T1b))"
+      and "\<forall> mb :: Ballot. MaxBal (f i) a mb \<longrightarrow> mb < b"
+      and "queued_msg (f i) a = None"
+      and "\<not> two_a_lrn_loop (f i) a"
+    shows "i < j \<and> M1a b \<notin> set (known_msgs_acc (f j) a) \<and>
+           (\<forall> k. i \<le> k \<and> k \<le> j \<longrightarrow> \<not> ProposerSendAction (f k) (f (1 + k))
+                                      \<and> \<not> FakeAcceptorAction (f k) (f (1 + k)))
+           \<longrightarrow>
+           (\<forall> k. i \<le> k \<and> k \<le> j \<longrightarrow> \<not> (\<exists>M \<in> set (msgs (f k)). M \<noteq> M1a b \<and> Recv_acc (f k) a M \<and> (type M = T1a \<or> type M = T1b))
+                                    \<and> (\<forall> mb :: Ballot. MaxBal (f k) a mb \<longrightarrow> mb < b)
+                                    \<and> queued_msg (f k) a = None
+                                    \<and> \<not> two_a_lrn_loop (f k) a)"
+proof (induction j)
+  case 0
+  then show ?case
+    by fastforce
+next
+  case (Suc j)
+  assume ih:"i < j \<and>
+         M1a b \<notin> set (known_msgs_acc (f j) a) \<and>
+         (\<forall>k. i \<le> k \<and> k \<le> j \<longrightarrow>
+              \<not> ProposerSendAction (f k) (f (1 + k)) \<and>
+              \<not> FakeAcceptorAction (f k) (f (1 + k))) \<longrightarrow>
+         (\<forall>k. i \<le> k \<and> k \<le> j \<longrightarrow>
+              \<not> (\<exists>M\<in>set (msgs (f k)).
+                     M \<noteq> M1a b \<and>
+                     Recv_acc (f k) a M \<and> (type M = T1a \<or> type M = T1b)) \<and>
+              (\<forall>mb. MaxBal (f k) a mb \<longrightarrow> mb < b)
+                                    \<and> queued_msg (f k) a = None
+                                    \<and> \<not> two_a_lrn_loop (f k) a)"
+  then show ?case
+  proof (clarify)
+    fix k
+    assume "i < Suc j"
+       and "M1a b \<notin> set (known_msgs_acc (f (Suc j)) a)"
+       and "\<forall>k. i \<le> k \<and> k \<le> Suc j \<longrightarrow>
+             \<not> ProposerSendAction (f k) (f (1 + k)) \<and>
+             \<not> FakeAcceptorAction (f k) (f (1 + k))"
+       and "i \<le> k"
+       and "k \<le> Suc j"
+    have "M1a b \<notin> set (known_msgs_acc (f j) a)"
+      by (metis \<open>M1a b \<notin> set (known_msgs_acc (f (Suc j)) a)\<close> assms(1) known_msgs_acc_preserved le_add2 plus_1_eq_Suc)
+    have "(\<forall>k. i \<le> k \<and> k \<le> j \<longrightarrow>
+              \<not> ProposerSendAction (f k) (f (1 + k)) \<and>
+              \<not> FakeAcceptorAction (f k) (f (1 + k)))"
+      using \<open>\<forall>k. i \<le> k \<and> k \<le> Suc j \<longrightarrow> \<not> ProposerSendAction (f k) (f (1 + k)) \<and> \<not> FakeAcceptorAction (f k) (f (1 + k))\<close> le_Suc_eq by presburger
+    have ihu:"(\<forall>k. i \<le> k \<and> k \<le> j \<longrightarrow>
+              \<not> (\<exists>M\<in>set (msgs (f k)).
+                     M \<noteq> M1a b \<and>
+                     Recv_acc (f k) a M \<and> (type M = T1a \<or> type M = T1b)) \<and>
+              (\<forall>mb. MaxBal (f k) a mb \<longrightarrow> mb < b))"
+      by (metis \<open>M1a b \<notin> set (known_msgs_acc (f j) a)\<close> \<open>\<forall>k. i \<le> k \<and> k \<le> j \<longrightarrow> \<not> ProposerSendAction (f k) (f (1 + k)) \<and> \<not> FakeAcceptorAction (f k) (f (1 + k))\<close> \<open>i < Suc j\<close> antisym assms(5) assms(6) ih less_SucE)
+    show "\<not> (\<exists>M\<in>set (msgs (f k)).
+                    M \<noteq> M1a b \<and>
+                    Recv_acc (f k) a M \<and> (type M = T1a \<or> type M = T1b))
+               \<and> (\<forall>mb. MaxBal (f k) a mb \<longrightarrow> mb < b)
+                                    \<and> queued_msg (f k) a = None
+                                    \<and> \<not> two_a_lrn_loop (f k) a"
+    proof (cases "k \<noteq> Suc j")
+      case True
+      then show ?thesis 
+        using \<open>\<forall>k. i \<le> k \<and> k \<le> j \<longrightarrow> \<not> (\<exists>M\<in>set (msgs (f k)). M \<noteq> M1a b \<and> Recv_acc (f k) a M \<and> (type M = T1a \<or> type M = T1b)) \<and> (\<forall>mb. MaxBal (f k) a mb \<longrightarrow> mb < b)\<close> \<open>i \<le> k\<close> \<open>k \<le> Suc j\<close> le_SucE by blast
+    next
+      case False
+      have ihu1: "\<not> (\<exists>M\<in>set (msgs (f j)).
+                     M \<noteq> M1a b \<and>
+                     Recv_acc (f j) a M \<and> (type M = T1a \<or> type M = T1b))"
+        using \<open>i < Suc j\<close> ihu less_Suc_eq_le by blast
+      have ihu2: "(\<forall>mb. MaxBal (f j) a mb \<longrightarrow> mb < b)"
+        using \<open>i < Suc j\<close> ihu less_Suc_eq_le by blast
+      have r1: "known_msgs_acc (f j) a = known_msgs_acc (f (Suc j)) a \<longrightarrow> (\<forall>mb. MaxBal (f k) a mb \<longrightarrow> mb < b)"
+        using False MaxBal.simps ihu2 by presburger
+      have r2: "known_msgs_acc (f j) a = known_msgs_acc (f (Suc j)) a \<and> set (msgs (f j)) = set (msgs (f (Suc j))) 
+            \<longrightarrow> \<not> (\<exists>M\<in>set (msgs (f k)). M \<noteq> M1a b \<and> Recv_acc (f k) a M \<and> (type M = T1a \<or> type M = T1b))"
+        unfolding Recv_acc.simps Proper_acc.simps
+        by (metis False Proper_acc.elims(1) Recv_acc.elims(3) Wellformed_Constant assms(1) ihu1)
+      have r3: "queued_msg (f j) a = queued_msg (f (Suc j)) a \<longrightarrow> queued_msg (f k) a = None"
+        by (metis False MessageType.distinct(1) QueuedMsgResult QueuedMsgSpec1.elims(2) QueuedMsgSpec2.elims(2) QueuedMsgSpec2_Conserved assms(1) assms(3) ihu1 type.simps(1))
+      have r4: "two_a_lrn_loop (f j) a = two_a_lrn_loop (f (Suc j)) a \<longrightarrow> \<not> two_a_lrn_loop (f k) a "
+        by (metis False Orderings.order_eq_iff \<open>M1a b \<notin> set (known_msgs_acc (f j) a)\<close> \<open>\<forall>k. i \<le> k \<and> k \<le> j \<longrightarrow> \<not> ProposerSendAction (f k) (f (1 + k)) \<and> \<not> FakeAcceptorAction (f k) (f (1 + k))\<close> \<open>i < Suc j\<close> assms(8) ih not_less_less_Suc_eq order_less_imp_le)
+      show ?thesis
+      proof (cases "f j = f (Suc j)")
+        case True
+        then show ?thesis
+          by (metis False \<open>M1a b \<notin> set (known_msgs_acc (f j) a)\<close> \<open>\<forall>k. i \<le> k \<and> k \<le> j \<longrightarrow> \<not> ProposerSendAction (f k) (f (1 + k)) \<and> \<not> FakeAcceptorAction (f k) (f (1 + k))\<close> \<open>i < Suc j\<close> assms(7) assms(8) dual_order.eq_iff dual_order.strict_implies_order ih not_less_less_Suc_eq r1 r2)
+      next
+        case False
+        have "Next (f j) (f (Suc j))"
+          using False Spec.simps assms(1) by blast
+        have "\<not> (ProposerSendAction (f j) (f (Suc j)))"
+          by (metis \<open>\<forall>k. i \<le> k \<and> k \<le> Suc j \<longrightarrow> \<not> ProposerSendAction (f k) (f (1 + k)) \<and> \<not> FakeAcceptorAction (f k) (f (1 + k))\<close> \<open>i < Suc j\<close> le_add2 less_Suc_eq_le plus_1_eq_Suc)
+        have "\<not> (FakeAcceptorAction (f j) (f (Suc j)))"
+          by (metis \<open>\<forall>k. i \<le> k \<and> k \<le> Suc j \<longrightarrow> \<not> ProposerSendAction (f k) (f (1 + k)) \<and> \<not> FakeAcceptorAction (f k) (f (1 + k))\<close> \<open>i < Suc j\<close> le_add2 less_Suc_eq_le plus_1_eq_Suc)
+        have "\<forall>m \<in> set (msgs (f j)). \<not> (Process1a a m (f j) (f (Suc j)))"
+          by (metis Process1a.elims(2) Process1a_Req_known_msgs \<open>M1a b \<notin> set (known_msgs_acc (f (Suc j)) a)\<close> assms(1) diff_Suc_1 ihu1)
+        have "\<forall>m \<in> set (msgs (f j)). \<not> (Process1b a m (f j) (f (Suc j)))"
+          by (metis Enabled.simps MessageType.distinct(1) Process1b_Enabled ihu1 type.simps(1))
+        then show ?thesis
+        proof (cases "LearnerProcessAction (f j) (f (Suc j))")
+          case True
+          then show ?thesis
+            unfolding LearnerProcessAction.simps LearnerAction.simps
+          proof (clarify)
+            fix ln
+            assume "(\<exists>m\<in>set (msgs (f j)). LearnerRecv ln m (f j) (f (Suc j))) \<or>
+                    (\<exists>blt val. LearnerDecide ln blt val (f j) (f (Suc j)))"
+            then show ?thesis
+              unfolding LearnerRecv.simps LearnerDecide.simps
+            proof -
+              assume a1: "(\<exists>m\<in>set (msgs (f j)). Recv_lrn (f j) ln m \<and> f (Suc j) = f j \<lparr>known_msgs_lrn := \<lambda>x. if ln = x then m # known_msgs_lrn (f j) x else known_msgs_lrn (f j) x\<rparr>) \<or> (\<exists>blt val. ChosenIn (f j) ln blt val \<and> f (Suc j) = f j \<lparr>decision := \<lambda>x y. if x = ln \<and> y = blt then {val} \<union> decision (f j) x y else decision (f j) x y\<rparr>)"
+              have "i < j \<and> M1a b \<notin> set (known_msgs_acc (f j) a) \<and> (\<forall>n. i \<le> n \<and> n \<le> j \<longrightarrow> \<not> ProposerSendAction (f n) (f (1 + n)) \<and> \<not> FakeAcceptorAction (f n) (f (1 + n))) \<longrightarrow> (\<forall>n. i \<le> n \<and> n \<le> j \<longrightarrow> (\<forall>p. p \<notin> set (msgs (f n)) \<or> p = M1a b \<or> \<not> Recv_acc (f n) a p \<or> type p \<noteq> T1a \<and> type p \<noteq> T1b) \<and> (\<forall>na. MaxBal (f n) a na \<longrightarrow> na < b) \<and> queued_msg (f n) a = None \<and> \<not> two_a_lrn_loop (f n) a)"
+                using ih by blast
+              then have f2: "\<not> i < j \<or> (\<forall>n. \<not> i \<le> n \<or> \<not> n \<le> j \<or> (\<forall>p. p \<notin> set (msgs (f n)) \<or> p = M1a b \<or> \<not> Recv_acc (f n) a p \<or> type p \<noteq> T1a \<and> type p \<noteq> T1b) \<and> (\<forall>na. \<not> MaxBal (f n) a na \<or> na < b) \<and> queued_msg (f n) a = None \<and> \<not> two_a_lrn_loop (f n) a)"
+                using \<open>M1a b \<notin> set (known_msgs_acc (f j) a)\<close> \<open>\<forall>k. i \<le> k \<and> k \<le> j \<longrightarrow> \<not> ProposerSendAction (f k) (f (1 + k)) \<and> \<not> FakeAcceptorAction (f k) (f (1 + k))\<close> by presburger
+              have f3: "\<forall>n na. n < na \<or> \<not> n < Suc na \<or> na = n"
+                using less_antisym by blast
+              then have f4: "i < j \<or> j = i"
+                using \<open>i < Suc j\<close> by blast
+              have f5: "k < Suc j \<or> Suc j = k"
+                using f3 \<open>k \<le> Suc j\<close> less_Suc_eq_le by blast
+              obtain nn :: nat and pp :: PreMessage where
+                f6: "((\<exists>p. p \<in> set (msgs (f k)) \<and> p \<noteq> M1a b \<and> Recv_acc (f k) a p \<and> (type p = T1a \<or> type p = T1b)) \<or> (\<exists>n. MaxBal (f k) a n \<and> \<not> n < b) \<or> queued_msg (f k) a \<noteq> None \<or> two_a_lrn_loop (f k) a) = (pp \<in> set (msgs (f k)) \<and> pp \<noteq> M1a b \<and> Recv_acc (f k) a pp \<and> (type pp = T1a \<or> type pp = T1b) \<or> MaxBal (f k) a nn \<and> \<not> nn < b \<or> queued_msg (f k) a \<noteq> None \<or> two_a_lrn_loop (f k) a)"
+                by blast
+              have f7: "\<lparr>msgs = msgs (f j), known_msgs_acc = known_msgs_acc (f j), known_msgs_lrn = \<lambda>l. if ln = l then v0_2 # known_msgs_lrn (f j) l else known_msgs_lrn (f j) l, recent_msgs = recent_msgs (f j), queued_msg = queued_msg (f j), two_a_lrn_loop = two_a_lrn_loop (f j), processed_lrns = processed_lrns (f j), decision = decision (f j), BVal = BVal (f j), \<dots> = more (f j)\<rparr> = f j\<lparr>known_msgs_lrn := \<lambda>l. if ln = l then v0_2 # known_msgs_lrn (f j) l else known_msgs_lrn (f j) l\<rparr>"
+                by simp
+              obtain ppa :: PreMessage and nna :: nat and vv :: Value where
+                f8: "ppa \<in> set (msgs (f j)) \<and> Recv_lrn (f j) ln ppa \<and> f (Suc j) = f j \<lparr>known_msgs_lrn := \<lambda>l. if ln = l then ppa # known_msgs_lrn (f j) l else known_msgs_lrn (f j) l\<rparr> \<or> ChosenIn (f j) ln nna vv \<and> f (Suc j) = f j \<lparr>decision := \<lambda>l n. if l = ln \<and> n = nna then {vv} \<union> decision (f j) l n else decision (f j) l n\<rparr>"
+                using a1 by blast
+              have f9: "f (Suc j) = f j \<lparr>decision := \<lambda>l n. if l = ln \<and> n = nna then {vv} \<union> decision (f j) l n else decision (f j) l n\<rparr> \<longrightarrow> \<lparr>msgs = msgs (f j), known_msgs_acc = known_msgs_acc (f j), known_msgs_lrn = known_msgs_lrn (f j), recent_msgs = recent_msgs (f j), queued_msg = queued_msg (f j), two_a_lrn_loop = two_a_lrn_loop (f j), processed_lrns = processed_lrns (f j), decision = \<lambda>l n. if l = ln \<and> n = nna then {vv} \<union> decision (f j) l n else decision (f j) l n, BVal = BVal (f j), \<dots> = more (f j)\<rparr> = \<lparr>msgs = msgs (f (Suc j)), known_msgs_acc = known_msgs_acc (f (Suc j)), known_msgs_lrn = known_msgs_lrn (f (Suc j)), recent_msgs = recent_msgs (f (Suc j)), queued_msg = queued_msg (f (Suc j)), two_a_lrn_loop = two_a_lrn_loop (f (Suc j)), processed_lrns = processed_lrns (f (Suc j)), decision = decision (f (Suc j)), BVal = BVal (f (Suc j)), \<dots> = more (f (Suc j))\<rparr>"
+                by simp
+              have f10: "\<forall>ps f fa fb fc p fd fe ff u psa fg fh fi fj pa fk fl fm ua. (\<lparr>msgs = ps, known_msgs_acc = f, known_msgs_lrn = fa, recent_msgs = fb, queued_msg = fc, two_a_lrn_loop = p, processed_lrns = fd, decision = fe, BVal = ff, \<dots> = u::unit\<rparr> = \<lparr>msgs = psa, known_msgs_acc = fg, known_msgs_lrn = fh, recent_msgs = fi, queued_msg = fj, two_a_lrn_loop = pa, processed_lrns = fk, decision = fl, BVal = fm, \<dots> = ua\<rparr>) = (ps = psa \<and> f = fg \<and> fa = fh \<and> fb = fi \<and> fc = fj \<and> p = pa \<and> fd = fk \<and> fe = fl \<and> ff = fm \<and> u = ua)"
+                by simp
+              have f11: "i \<le> j"
+                using \<open>i < Suc j\<close> by auto
+              have f12: "queued_msg (f j) = queued_msg (f (Suc j)) \<and> queued_msg (f k) a \<noteq> None \<longrightarrow> queued_msg (f k) a = None"
+                using f4 f3 f2 by (metis (no_types) \<open>i \<le> k\<close> \<open>k \<le> Suc j\<close> assms(7) less_Suc_eq_le linorder_not_less)
+              moreover
+              { assume "ppa \<notin> set (msgs (f j)) \<or> \<not> Recv_lrn (f j) ln ppa \<or> f (Suc j) \<noteq> f j \<lparr>known_msgs_lrn := \<lambda>l. if ln = l then ppa # known_msgs_lrn (f j) l else known_msgs_lrn (f j) l\<rparr>"
+                moreover
+                { assume "(msgs (f j) = msgs (f (Suc j)) \<and> known_msgs_acc (f j) = known_msgs_acc (f (Suc j)) \<and> known_msgs_lrn (f j) = known_msgs_lrn (f (Suc j)) \<and> recent_msgs (f j) = recent_msgs (f (Suc j)) \<and> queued_msg (f j) = queued_msg (f (Suc j)) \<and> two_a_lrn_loop (f j) = two_a_lrn_loop (f (Suc j)) \<and> processed_lrns (f j) = processed_lrns (f (Suc j)) \<and> (\<lambda>l n. if l = ln \<and> n = nna then {vv} \<union> decision (f j) l n else decision (f j) l n) = decision (f (Suc j)) \<and> BVal (f j) = BVal (f (Suc j)) \<and> more (f j) = more (f (Suc j))) \<and> \<not> two_a_lrn_loop (f (Suc j)) a"
+                  then have "(msgs (f j) = msgs (f (Suc j)) \<and> known_msgs_acc (f j) = known_msgs_acc (f (Suc j)) \<and> known_msgs_lrn (f j) = known_msgs_lrn (f (Suc j)) \<and> recent_msgs (f j) = recent_msgs (f (Suc j)) \<and> queued_msg (f j) = queued_msg (f (Suc j)) \<and> two_a_lrn_loop (f j) = two_a_lrn_loop (f (Suc j)) \<and> processed_lrns (f j) = processed_lrns (f (Suc j)) \<and> (\<lambda>l n. if l = ln \<and> n = nna then {vv} \<union> decision (f j) l n else decision (f j) l n) = decision (f (Suc j)) \<and> BVal (f j) = BVal (f (Suc j)) \<and> more (f j) = more (f (Suc j))) \<and> Suc j \<noteq> k \<or> (msgs (f j) = msgs (f (Suc j)) \<and> known_msgs_acc (f j) = known_msgs_acc (f (Suc j)) \<and> known_msgs_lrn (f j) = known_msgs_lrn (f (Suc j)) \<and> recent_msgs (f j) = recent_msgs (f (Suc j)) \<and> queued_msg (f j) = queued_msg (f (Suc j)) \<and> two_a_lrn_loop (f j) = two_a_lrn_loop (f (Suc j)) \<and> processed_lrns (f j) = processed_lrns (f (Suc j)) \<and> (\<lambda>l n. if l = ln \<and> n = nna then {vv} \<union> decision (f j) l n else decision (f j) l n) = decision (f (Suc j)) \<and> BVal (f j) = BVal (f (Suc j)) \<and> more (f j) = more (f (Suc j))) \<and> \<not> two_a_lrn_loop (f k) a"
+                    by meson }
+                moreover
+                { assume "(msgs (f j) = msgs (f (Suc j)) \<and> known_msgs_acc (f j) = known_msgs_acc (f (Suc j)) \<and> known_msgs_lrn (f j) = known_msgs_lrn (f (Suc j)) \<and> recent_msgs (f j) = recent_msgs (f (Suc j)) \<and> queued_msg (f j) = queued_msg (f (Suc j)) \<and> two_a_lrn_loop (f j) = two_a_lrn_loop (f (Suc j)) \<and> processed_lrns (f j) = processed_lrns (f (Suc j)) \<and> (\<lambda>l n. if l = ln \<and> n = nna then {vv} \<union> decision (f j) l n else decision (f j) l n) = decision (f (Suc j)) \<and> BVal (f j) = BVal (f (Suc j)) \<and> more (f j) = more (f (Suc j))) \<and> \<not> j \<le> j"
+                  then have "(msgs (f j) = msgs (f (Suc j)) \<and> known_msgs_acc (f j) = known_msgs_acc (f (Suc j)) \<and> known_msgs_lrn (f j) = known_msgs_lrn (f (Suc j)) \<and> recent_msgs (f j) = recent_msgs (f (Suc j)) \<and> queued_msg (f j) = queued_msg (f (Suc j)) \<and> two_a_lrn_loop (f j) = two_a_lrn_loop (f (Suc j)) \<and> processed_lrns (f j) = processed_lrns (f (Suc j)) \<and> (\<lambda>l n. if l = ln \<and> n = nna then {vv} \<union> decision (f j) l n else decision (f j) l n) = decision (f (Suc j)) \<and> BVal (f j) = BVal (f (Suc j)) \<and> more (f j) = more (f (Suc j))) \<and> Suc j \<noteq> k \<or> (msgs (f j) = msgs (f (Suc j)) \<and> known_msgs_acc (f j) = known_msgs_acc (f (Suc j)) \<and> known_msgs_lrn (f j) = known_msgs_lrn (f (Suc j)) \<and> recent_msgs (f j) = recent_msgs (f (Suc j)) \<and> queued_msg (f j) = queued_msg (f (Suc j)) \<and> two_a_lrn_loop (f j) = two_a_lrn_loop (f (Suc j)) \<and> processed_lrns (f j) = processed_lrns (f (Suc j)) \<and> (\<lambda>l n. if l = ln \<and> n = nna then {vv} \<union> decision (f j) l n else decision (f j) l n) = decision (f (Suc j)) \<and> BVal (f j) = BVal (f (Suc j)) \<and> more (f j) = more (f (Suc j))) \<and> k \<le> j"
+                    by force }
+                ultimately have "(msgs (f j) = msgs (f (Suc j)) \<and> known_msgs_acc (f j) = known_msgs_acc (f (Suc j)) \<and> known_msgs_lrn (f j) = known_msgs_lrn (f (Suc j)) \<and> recent_msgs (f j) = recent_msgs (f (Suc j)) \<and> queued_msg (f j) = queued_msg (f (Suc j)) \<and> two_a_lrn_loop (f j) = two_a_lrn_loop (f (Suc j)) \<and> processed_lrns (f j) = processed_lrns (f (Suc j)) \<and> (\<lambda>l n. if l = ln \<and> n = nna then {vv} \<union> decision (f j) l n else decision (f j) l n) = decision (f (Suc j)) \<and> BVal (f j) = BVal (f (Suc j)) \<and> more (f j) = more (f (Suc j))) \<and> Suc j \<noteq> k \<or> (msgs (f j) = msgs (f (Suc j)) \<and> known_msgs_acc (f j) = known_msgs_acc (f (Suc j)) \<and> known_msgs_lrn (f j) = known_msgs_lrn (f (Suc j)) \<and> recent_msgs (f j) = recent_msgs (f (Suc j)) \<and> queued_msg (f j) = queued_msg (f (Suc j)) \<and> two_a_lrn_loop (f j) = two_a_lrn_loop (f (Suc j)) \<and> processed_lrns (f j) = processed_lrns (f (Suc j)) \<and> (\<lambda>l n. if l = ln \<and> n = nna then {vv} \<union> decision (f j) l n else decision (f j) l n) = decision (f (Suc j)) \<and> BVal (f j) = BVal (f (Suc j)) \<and> more (f j) = more (f (Suc j))) \<and> k \<le> j \<or> (msgs (f j) = msgs (f (Suc j)) \<and> known_msgs_acc (f j) = known_msgs_acc (f (Suc j)) \<and> known_msgs_lrn (f j) = known_msgs_lrn (f (Suc j)) \<and> recent_msgs (f j) = recent_msgs (f (Suc j)) \<and> queued_msg (f j) = queued_msg (f (Suc j)) \<and> two_a_lrn_loop (f j) = two_a_lrn_loop (f (Suc j)) \<and> processed_lrns (f j) = processed_lrns (f (Suc j)) \<and> (\<lambda>l n. if l = ln \<and> n = nna then {vv} \<union> decision (f j) l n else decision (f j) l n) = decision (f (Suc j)) \<and> BVal (f j) = BVal (f (Suc j)) \<and> more (f j) = more (f (Suc j))) \<and> j = i \<or> (msgs (f j) = msgs (f (Suc j)) \<and> known_msgs_acc (f j) = known_msgs_acc (f (Suc j)) \<and> known_msgs_lrn (f j) = known_msgs_lrn (f (Suc j)) \<and> recent_msgs (f j) = recent_msgs (f (Suc j)) \<and> queued_msg (f j) = queued_msg (f (Suc j)) \<and> two_a_lrn_loop (f j) = two_a_lrn_loop (f (Suc j)) \<and> processed_lrns (f j) = processed_lrns (f (Suc j)) \<and> (\<lambda>l n. if l = ln \<and> n = nna then {vv} \<union> decision (f j) l n else decision (f j) l n) = decision (f (Suc j)) \<and> BVal (f j) = BVal (f (Suc j)) \<and> more (f j) = more (f (Suc j))) \<and> \<not> two_a_lrn_loop (f k) a"
+                  using f11 f10 f9 f8 f4 f2 by (smt (z3))
+                then have "(pp \<notin> set (msgs (f k)) \<or> pp = M1a b \<or> \<not> Recv_acc (f k) a pp \<or> type pp \<noteq> T1a \<and> type pp \<noteq> T1b) \<and> (\<not> MaxBal (f k) a nn \<or> nn < b) \<and> queued_msg (f k) a = None \<and> \<not> two_a_lrn_loop (f k) a"
+                  using f12 f5 f4 f3 f2 by (smt (z3) \<open>i \<le> k\<close> assms(8) less_Suc_eq_le linorder_not_less r1 r2) }
+              ultimately show ?thesis
+                using f10 f7 f6 f5 f4 f3 f2
+                by (smt (z3) \<open>i \<le> k\<close> assms(8) less_Suc_eq_le linorder_not_less r1 r2 surjective update_convs(3))
+            qed
+          qed
+        next
+          case False
+          have "AcceptorProcessAction (f j) (f (Suc j))"
+            using False Next.elims(2) \<open>Next (f j) (f (Suc j))\<close> \<open>\<not> FakeAcceptorAction (f j) (f (Suc j))\<close> \<open>\<not> ProposerSendAction (f j) (f (Suc j))\<close> by blast
+          then have "(\<exists>A :: Acceptor. is_safe A
+                                    \<and> queued_msg (f j) A = None 
+                                    \<and> (\<exists>m \<in> set (msgs (f j)). Process1a A m (f j) (f (Suc j)))) \<or>
+                      (\<exists>A :: Acceptor. is_safe A
+                                    \<and> queued_msg (f j) A \<noteq> None 
+                                    \<and> Process1b A (the (queued_msg (f j) A)) (f j) (f (Suc j))) \<or>
+                      (\<exists>A :: Acceptor. is_safe A
+                                    \<and> queued_msg (f j) A = None 
+                                    \<and> (\<exists>m \<in> set (msgs (f j)). Process1b A m (f j) (f (Suc j)))) \<or>
+                      (\<exists>A :: Acceptor. is_safe A
+                                    \<and> two_a_lrn_loop (f j) A 
+                                    \<and> (\<exists>l :: Learner. Process1bLearnerLoopStep A l (f j) (f (Suc j)))) \<or>
+                      (\<exists>A :: Acceptor. is_safe A
+                                    \<and> two_a_lrn_loop (f j) A 
+                                    \<and> Process1bLearnerLoopDone A (f j) (f (Suc j)))"
+            using Acceptor_split by presburger
+          then show ?thesis
+          proof (elim disjE)
+            assume "\<exists>A. is_safe A \<and>
+              queued_msg (f j) A = None \<and>
+              (\<exists>m\<in>set (msgs (f j)).
+                  Process1a A m (f j) (f (Suc j)))"
+            then show ?thesis
+            proof (clarify)
+              fix A m
+              assume "is_safe A"
+                 and "queued_msg (f j) A = None"
+                 and "m \<in> set (msgs (f j))"
+                 and "Process1a A m (f j) (f (Suc j))"
+              define new1b where "new1b = M1b A (m # recent_msgs (f j) A)"
+              have "WellFormed (f j) new1b"
+                sorry
+              then show ?thesis
+                sorry
+            qed
+          next
+            assume "\<exists>A. is_safe A \<and>
+                      queued_msg (f j) A \<noteq> None \<and>
+                      Process1b A (the (queued_msg (f j) A)) (f j) (f (Suc j))"
+            then show ?thesis
+            proof (clarify)
+              fix A y
+              assume "is_safe A"
+                 and "queued_msg (f j) A = Some y"
+                 and "Process1b A (the (queued_msg (f j) A)) (f j) (f (Suc j))"
+              then show ?thesis
+                unfolding Process1b.simps
+                sorry
+            qed
+          next
+            assume "\<exists>A. is_safe A \<and>
+                        queued_msg (f j) A = None \<and>
+                        (\<exists>m\<in>set (msgs (f j)). Process1b A m (f j) (f (Suc j)))"
+            then show ?thesis
+            proof (clarify)
+              fix A m
+              assume "is_safe A"
+                 and "queued_msg (f j) A = None"
+                 and "m\<in>set (msgs (f j))"
+                 and "Process1b A m (f j) (f (Suc j))"
+              then have "A \<noteq> a"
+                sorry
+              then show ?thesis
+                sorry
+            qed
+          next
+            assume "\<exists>A. is_safe A \<and>
+                two_a_lrn_loop (f j) A \<and>
+                (\<exists>l. Process1bLearnerLoopStep A l (f j) (f (Suc j)))"
+            then show ?thesis
+            proof (clarify)
+              fix A l
+              assume "is_safe A"
+                 and "two_a_lrn_loop (f j) A"
+                 and "Process1bLearnerLoopStep A l (f j) (f (Suc j))"
+              then have "A \<noteq> a"
+                sorry
+              then show ?thesis
+                sorry
+            qed
+          next
+            assume "\<exists>A. is_safe A \<and>
+                      two_a_lrn_loop (f j) A \<and>
+                      Process1bLearnerLoopDone A (f j) (f (Suc j))"
+            then show ?thesis
+            proof (clarify)
+              fix A
+              assume "is_safe A"
+                 and "two_a_lrn_loop (f j) A"
+                 and "Process1bLearnerLoopDone A (f j) (f (Suc j))"
+              then have "A \<noteq> a"
+                sorry
+              then show ?thesis
+                sorry
+            qed
+          qed
+        qed
+      qed
+    qed
+  qed
+qed
+
+lemma step_1a_full:
+  assumes "Spec f"
+      and "M1a b \<in> set (msgs (f i))"
+      and "\<forall> mb :: Ballot. MaxBal (f i) a mb \<longrightarrow> mb < b"
+      and "is_safe a"
+      and "M1a b \<notin> set (known_msgs_acc (f i) a)"
+      and "\<not> (\<exists>M \<in> set (msgs (f i)). M \<noteq> M1a b \<and> Recv_acc (f i) a M \<and> (type M = T1a \<or> type M = T1b))"
+    shows "M1a b \<in> set (known_msgs_acc (f (i + j)) a) \<and>
+           (\<forall> k. i \<le> k \<and> k \<le> i + j \<longrightarrow> \<not> ProposerSendAction (f k) (f (1 + k))
+                                      \<and> \<not> FakeAcceptorAction (f k) (f (1 + k)))
+           \<longrightarrow>
+           (\<exists>k. i \<le> k \<and> k < i + j \<and>
+             (\<forall> mb :: Ballot. MaxBal (f k) a mb \<longrightarrow> mb < b) \<and>
+             \<not> (\<exists>M \<in> set (msgs (f k)). M \<noteq> M1a b \<and> Recv_acc (f k) a M \<and> (type M = T1a \<or> type M = T1b)))"
+proof (induction j)
+  case 0
+  then show ?case
+    by (metis assms(5) verit_sum_simplify)
+next
+  case (Suc j)
+  then show ?case sorry
+qed
+
+lemma step_:
+  assumes "Spec f"
+      and "M1a b \<in> set (msgs (f i))"
+      and "\<forall> mb :: Ballot. MaxBal (f i) a mb \<longrightarrow> mb < b"
+      and "is_safe a"
+      and "M1a b \<notin> set (known_msgs_acc (f i) a)"
+      and "\<not> (\<exists>M \<in> set (msgs (f i)). M \<noteq> M1a b \<and> Recv_acc (f i) a M \<and> (type M = T1a \<or> type M = T1b))"
+    shows "i < j \<and> M1a b \<in> set (known_msgs_acc (f j) a) \<and>
+           (\<forall> k. i < k \<and> k < j \<longrightarrow> \<not> ProposerSendAction (f k) (f (1 + k))
+                                 \<and> \<not> FakeAcceptorAction (f k) (f (1 + k)))
+           \<longrightarrow>
+           (\<exists>k. i \<le> k \<and> k < j \<and> 
+             M1a b \<notin> set (known_msgs_acc (f k) a) \<and>
+             Process1a a (M1a b) (f k) (f (1 + k)) \<and>
+             (\<forall> mb :: Ballot. MaxBal (f k) a mb \<longrightarrow> mb < b) \<and>
+             \<not> (\<exists>M \<in> set (msgs (f k)). M \<noteq> M1a b \<and> Recv_acc (f k) a M \<and> (type M = T1a \<or> type M = T1b)))"
+proof (induction j)
+  case 0
+  then show ?case 
+    by fastforce
+next
+  case (Suc j)
+  assume ih: "i < j \<and>
+         M1a b \<in> set (known_msgs_acc (f j) a) \<and>
+         (\<forall>k. i < k \<and> k < j \<longrightarrow>
+              \<not> ProposerSendAction (f k) (f (1 + k)) \<and>
+              \<not> FakeAcceptorAction (f k) (f (1 + k))) \<longrightarrow>
+         (\<exists>k\<ge>i. k < j \<and>
+                 M1a b \<notin> set (known_msgs_acc (f k) a) \<and>
+                 Process1a a (M1a b) (f k) (f (1 + k)) \<and>
+                 (\<forall>mb. MaxBal (f k) a mb \<longrightarrow> mb < b) \<and>
+                 \<not> (\<exists>M\<in>set (msgs (f k)).
+                        M \<noteq> M1a b \<and>
+                        Recv_acc (f k) a M \<and>
+                        (type M = T1a \<or> type M = T1b)))"
+  show ?case
+  proof (clarify)
+    assume "i < Suc j"
+       and "M1a b \<in> set (known_msgs_acc (f (Suc j)) a)"
+       and "\<forall>k. i < k \<and> k < Suc j \<longrightarrow>
+            \<not> ProposerSendAction (f k) (f (1 + k)) \<and>
+            \<not> FakeAcceptorAction (f k) (f (1 + k))"
+    then show "\<exists>k\<ge>i. k < Suc j \<and>
+           M1a b \<notin> set (known_msgs_acc (f k) a) \<and>
+           Process1a a (M1a b) (f k) (f (1 + k)) \<and>
+           (\<forall>mb. MaxBal (f k) a mb \<longrightarrow> mb < b) \<and>
+           \<not> (\<exists>M\<in>set (msgs (f k)).
+                  M \<noteq> M1a b \<and>
+                  Recv_acc (f k) a M \<and>
+                  (type M = T1a \<or> type M = T1b))"
+    proof (cases "i = j")
+      case True
+      then show ?thesis
+        by (metis \<open>M1a b \<in> set (known_msgs_acc (f (Suc j)) a)\<close> \<open>i < Suc j\<close> assms(1) assms(2) assms(3) assms(4) assms(5) assms(6) le_less_Suc_eq step_1a_only)
+    next
+      case False
+      have "i < j"
+        using False \<open>i < Suc j\<close> by linarith
+      have "(\<forall>k. i < k \<and> k < j \<longrightarrow>
+              \<not> ProposerSendAction (f k) (f (1 + k)) \<and>
+              \<not> FakeAcceptorAction (f k) (f (1 + k)))"
+        using \<open>\<forall>k. i < k \<and> k < Suc j \<longrightarrow> \<not> ProposerSendAction (f k) (f (1 + k)) \<and> \<not> FakeAcceptorAction (f k) (f (1 + k))\<close> less_Suc_eq by blast
+      then show ?thesis sorry
+    qed
+
+
+      proof (cases "M1a b \<in> set (known_msgs_acc (f j) a)")
+        case True
+        then show ?thesis
+          by (metis Suc \<open>\<forall>k. i < k \<and> k < Suc j \<longrightarrow> \<not> ProposerSendAction (f k) (f (1 + k)) \<and> \<not> FakeAcceptorAction (f k) (f (1 + k))\<close> \<open>i < Suc j\<close> assms(5) less_Suc_eq)
+      next
+        case False
+          have "Next (f j) (f (Suc j))"
+            by (metis False Spec.elims(2) \<open>M1a b \<in> set (known_msgs_acc (f (Suc j)) a)\<close> assms(1))
+          then have "\<not> (ProposerSendAction (f j) (f (Suc j)))"
+            by (metis False ProposerSendAction.elims(2) Send1a.elims(2) \<open>M1a b \<in> set (known_msgs_acc (f (Suc j)) a)\<close> ext_inject surjective update_convs(1))
+          have "\<forall> ln m. \<not> (LearnerRecv ln m (f j) (f (Suc j)))"
+            by (smt (verit, ccfv_SIG) False LearnerRecv.simps \<open>M1a b \<in> set (known_msgs_acc (f (Suc j)) a)\<close> ext_inject surjective update_convs(3))
+          have "\<forall> ln blt val. \<not> (LearnerDecide ln blt val (f j) (f (Suc j)))"
+            using False \<open>M1a b \<in> set (known_msgs_acc (f (Suc j)) a)\<close> by force
+          then have "\<forall>a. \<not> (LearnerProcessAction (f j) (f (Suc j)))"
+            by (meson LearnerAction.elims(2) LearnerProcessAction.elims(1) \<open>\<forall>ln m. \<not> LearnerRecv ln m (f j) (f (Suc j))\<close>)
+          have "\<forall>a. \<not> (FakeSend1b a (f j) (f (Suc j)))"
+            by (metis FakeSend1b.elims(1) False \<open>M1a b \<in> set (known_msgs_acc (f (Suc j)) a)\<close> ext_inject surjective update_convs(1))
+          have "\<forall>a. \<not> (FakeSend2a a (f j) (f (Suc j)))"
+            by (metis FakeSend2a.simps False \<open>M1a b \<in> set (known_msgs_acc (f (Suc j)) a)\<close> ext_inject surjective update_convs(1))
+          then have "\<not> (FakeAcceptorAction (f j) (f (Suc j)))"
+            using FakeAcceptorAction.simps \<open>\<forall>a. \<not> FakeSend1b a (f j) (f (Suc j))\<close> by presburger
+          then have "AcceptorProcessAction (f j) (f (Suc j))"
+            by (meson LearnerAction.elims(2) LearnerProcessAction.elims(2) Next.simps \<open>Next (f j) (f (Suc j))\<close> \<open>\<forall>ln blt val. \<not> LearnerDecide ln blt val (f j) (f (Suc j))\<close> \<open>\<forall>ln m. \<not> LearnerRecv ln m (f j) (f (Suc j))\<close> \<open>\<not> ProposerSendAction (f j) (f (Suc j))\<close>)
+          have "\<forall> A m. a \<noteq> A \<longrightarrow> \<not> (Process1a A m (f j) (f (Suc j)))"
+            by (metis False Process1a.elims(2) Store_acc.elims(2) \<open>M1a b \<in> set (known_msgs_acc (f (Suc j)) a)\<close>)
+          have "\<forall> A m. a \<noteq> A \<longrightarrow> \<not> (Process1b A m (f j) (f (Suc j)))"
+            by (metis False Process1b.elims(2) Store_acc.elims(2) \<open>M1a b \<in> set (known_msgs_acc (f (Suc j)) a)\<close>)
+          have "\<forall> a. \<not> (Process1bLearnerLoopDone a (f j) (f (Suc j)))"
+            using False \<open>M1a b \<in> set (known_msgs_acc (f (Suc j)) a)\<close> by force
+          have "\<forall> ln. \<not> (Process1bLearnerLoopStep a ln (f j) (f (Suc j)))"
+            unfolding Process1bLearnerLoopStep.simps
+            by (smt (verit, ccfv_SIG) False PreMessage.distinct(3) Store_acc.elims(2) \<open>M1a b \<in> set (known_msgs_acc (f (Suc j)) a)\<close> set_ConsD)  
+          then have "\<forall> A. a \<noteq> A \<longrightarrow> \<not> AcceptorAction A (f j) (f (Suc j))"
+          proof -
+            { fix aa :: Acceptor
+              have "known_msgs_acc (f (Suc j)) \<noteq> known_msgs_acc (f j) \<and> known_msgs_acc (f (Suc j)) a \<noteq> known_msgs_acc (f j) a"
+                using False \<open>M1a b \<in> set (known_msgs_acc (f (Suc j)) a)\<close> by fastforce
+              then have "aa = a \<or> \<not> AcceptorAction aa (f j) (f (Suc j))"
+                by (metis (full_types) AcceptorAction.elims(2) Process1bLearnerLoop.elims(2) Process1bLearnerLoopStep.elims(2) Store_acc.elims(2) \<open>\<forall>A m. a \<noteq> A \<longrightarrow> \<not> Process1a A m (f j) (f (Suc j))\<close> \<open>\<forall>A m. a \<noteq> A \<longrightarrow> \<not> Process1b A m (f j) (f (Suc j))\<close> \<open>\<forall>a. \<not> Process1bLearnerLoopDone a (f j) (f (Suc j))\<close>) }
+            then show ?thesis
+              by (metis (no_types))
+          qed
+          then have "AcceptorAction a (f j) (f (Suc j))"
+            by (metis AcceptorProcessAction.simps \<open>AcceptorProcessAction (f j) (f (Suc j))\<close>)
+          have "\<forall> m. (M1a b) \<noteq> m \<longrightarrow> \<not> (Process1a a m (f j) (f (Suc j)))"
+            unfolding Process1a.simps
+            by (metis False Store_acc.elims(2) \<open>M1a b \<in> set (known_msgs_acc (f (Suc j)) a)\<close> set_ConsD)
+          have "\<not> (Process1b a (M1a b) (f j) (f (Suc j)))"
+            by simp
+          have "\<forall> m. (M1a b) \<noteq> m \<longrightarrow> \<not> (Process1b a m (f j) (f (Suc j)))"
+            unfolding Process1b.simps
+            by (metis (no_types, lifting) False Store_acc.elims(2) \<open>M1a b \<in> set (known_msgs_acc (f (Suc j)) a)\<close> set_ConsD)
+          then have "\<forall> m. \<not> (Process1b a m (f j) (f (Suc j)))"
+            by (metis \<open>\<not> Process1b a (M1a b) (f j) (f (Suc j))\<close>)
+          then have "Process1a a (M1a b) (f j) (f (Suc j))"
+            by (metis AcceptorAction.elims(2) Process1bLearnerLoop.elims(2) \<open>AcceptorAction a (f j) (f (Suc j))\<close> \<open>\<forall>a. \<not> Process1bLearnerLoopDone a (f j) (f (Suc j))\<close> \<open>\<forall>ln. \<not> Process1bLearnerLoopStep a ln (f j) (f (Suc j))\<close> \<open>\<forall>m. M1a b \<noteq> m \<longrightarrow> \<not> Process1a a m (f j) (f (Suc j))\<close>)
+          then have "\<exists>k. i \<le> k \<and> k < Suc j \<and> Process1a a (M1a b) (f k) (f (1 + k))"
+            by (metis \<open>i < Suc j\<close> less_Suc_eq less_Suc_eq_le plus_1_eq_Suc)
+          have "\<forall>k. i < k \<and> k < j \<longrightarrow>
+              \<not> ProposerSendAction (f k) (f (1 + k)) \<and>
+              \<not> FakeAcceptorAction (f k) (f (1 + k))"
+            using \<open>\<forall>k. i < k \<and> k < Suc j \<longrightarrow> \<not> ProposerSendAction (f k) (f (1 + k)) \<and> \<not> FakeAcceptorAction (f k) (f (1 + k))\<close> less_Suc_eq by presburger
+          show ?thesis
+          proof (cases "i < j")
+            case True
+            have "\<exists>k\<ge>i. k < j \<and>
+                 Process1a a (M1a b) (f k) (f (1 + k)) \<and>
+                 (\<forall>mb. MaxBal (f k) a mb \<longrightarrow> mb < b) \<and>
+                 \<not> (\<exists>M\<in>set (msgs (f k)).
+                        M \<noteq> M1a b \<and>
+                        Recv_acc (f k) a M \<and>
+                        (type M = T1a \<or> type M = T1b))"
+              sorry
+            then show ?thesis sorry
+          next
+            case False
+            have "i = j"
+              using False \<open>i < Suc j\<close> less_Suc_eq by blast
+            then show ?thesis
+              using \<open>\<exists>k\<ge>i. k < Suc j \<and> Process1a a (M1a b) (f k) (f (1 + k))\<close> assms(3) assms(6) le_less_Suc_eq by blast
+          qed
+        qed
+      qed
+
+  qed
+qed
+*)
